checkpoint in ghc. Currently working on Class/DataCon/TyCon

examples/ghc/manual/DataCon.v
@@ -10,70 +10,247 @@ Unset Printing Implicit Defensive.
 Require Coq.Program.Tactics.
 Require Coq.Program.Wf.
 
-(* Preamble *)
-
-
 (* Converted imports: *)
 
 Require BasicTypes.
+Require Class.
 Require Coq.Init.Datatypes.
 Require Coq.Lists.List.
 Require Data.Foldable.
+Require Data.Set.Internal.
 Require Data.Traversable.
 Require Data.Tuple.
+Require FastString.
 Require FieldLabel.
+(* Require ForeignCall. *)
 Require GHC.Base.
+Require GHC.Err.
 Require GHC.List.
+Require GHC.Num.
+Require ListSetOps.
 Require Name.
-Require NameEnv.
-
-(* Require Var. *)
+Require OccName.
+Require Panic.
+Require PrelNames.
+(* Require TysWiredIn. *)
+Require UniqSet.
+Require Unique.
+Require Util.
 Import GHC.Base.Notations.
+Import GHC.Num.Notations.
 
 (* Converted type declarations: *)
 
-Inductive StrictnessMark : Type := MarkedStrict : StrictnessMark
-                                |  NotMarkedStrict : StrictnessMark.
+Inductive StrictnessMark : Type
+  := MarkedStrict : StrictnessMark
+  |  NotMarkedStrict : StrictnessMark.
 
-Inductive SrcUnpackedness : Type := SrcUnpack : SrcUnpackedness
-                                 |  SrcNoUnpack : SrcUnpackedness
-                                 |  NoSrcUnpack : SrcUnpackedness.
+Inductive SrcUnpackedness : Type
+  := SrcUnpack : SrcUnpackedness
+  |  SrcNoUnpack : SrcUnpackedness
+  |  NoSrcUnpack : SrcUnpackedness.
 
-Inductive SrcStrictness : Type := SrcLazy : SrcStrictness
-                               |  SrcStrict : SrcStrictness
-                               |  NoSrcStrict : SrcStrictness.
+Inductive SrcStrictness : Type
+  := SrcLazy : SrcStrictness
+  |  SrcStrict : SrcStrictness
+  |  NoSrcStrict : SrcStrictness.
 
-Inductive HsSrcBang : Type := Mk_HsSrcBang : (option BasicTypes.SourceText) -> SrcUnpackedness -> SrcStrictness -> HsSrcBang.
+Inductive HsSrcBang : Type
+  := Mk_HsSrcBang
+   : BasicTypes.SourceText -> SrcUnpackedness -> SrcStrictness -> HsSrcBang.
 
-Parameter HsImplBang : Type.
+Inductive HsImplBang : Type
+  := HsLazy : HsImplBang
+  |  HsStrict : HsImplBang
+  |  HsUnpack : (option unit) -> HsImplBang.
 
-Parameter EqSpec : Type.
+Inductive EqSpec : Type := Mk_EqSpec : Var.TyVar -> unit -> EqSpec.
 
-Parameter DataConRep : Type.
+Inductive DataConRep : Type
+  := NoDataConRep : DataConRep
+  |  DCR
+   : Var.Id ->
+     unit -> list unit -> list StrictnessMark -> list HsImplBang -> DataConRep.
 
-Parameter DataCon : Type.
+Inductive DataCon : Type
+  := MkData
+   : Name.Name ->
+     Unique.Unique ->
+     BasicTypes.ConTag ->
+     bool ->
+     list Var.TyVar ->
+     list Var.TyVar ->
+     list Var.TyVarBinder ->
+     list EqSpec ->
+     unit ->
+     unit ->
+     list unit ->
+     unit ->
+     list HsSrcBang ->
+     list FieldLabel.FieldLabel ->
+     Var.Id ->
+     DataConRep ->
+     BasicTypes.Arity -> BasicTypes.Arity -> unit -> unit -> bool -> unit -> DataCon.
+
+Instance Default__StrictnessMark : GHC.Err.Default StrictnessMark :=
+  GHC.Err.Build_Default _ MarkedStrict.
+
+Instance Default__SrcUnpackedness : GHC.Err.Default SrcUnpackedness :=
+  GHC.Err.Build_Default _ SrcUnpack.
+
+Instance Default__SrcStrictness : GHC.Err.Default SrcStrictness :=
+  GHC.Err.Build_Default _ SrcLazy.
+
+Instance Default__HsImplBang : GHC.Err.Default HsImplBang :=
+  GHC.Err.Build_Default _ HsLazy.
+
+Instance Default__DataConRep : GHC.Err.Default DataConRep :=
+  GHC.Err.Build_Default _ NoDataConRep.
+
+Definition dcr_arg_tys (arg_0__ : DataConRep) :=
+  match arg_0__ with
+  | NoDataConRep =>
+      GHC.Err.error (GHC.Base.hs_string__
+                     "Partial record selector: field `dcr_arg_tys' has no match in constructor `NoDataConRep' of type `DataConRep'")
+  | DCR _ _ dcr_arg_tys _ _ => dcr_arg_tys
+  end.
+
+Definition dcr_bangs (arg_0__ : DataConRep) :=
+  match arg_0__ with
+  | NoDataConRep =>
+      GHC.Err.error (GHC.Base.hs_string__
+                     "Partial record selector: field `dcr_bangs' has no match in constructor `NoDataConRep' of type `DataConRep'")
+  | DCR _ _ _ _ dcr_bangs => dcr_bangs
+  end.
+
+Definition dcr_boxer (arg_0__ : DataConRep) :=
+  match arg_0__ with
+  | NoDataConRep =>
+      GHC.Err.error (GHC.Base.hs_string__
+                     "Partial record selector: field `dcr_boxer' has no match in constructor `NoDataConRep' of type `DataConRep'")
+  | DCR _ dcr_boxer _ _ _ => dcr_boxer
+  end.
+
+Definition dcr_stricts (arg_0__ : DataConRep) :=
+  match arg_0__ with
+  | NoDataConRep =>
+      GHC.Err.error (GHC.Base.hs_string__
+                     "Partial record selector: field `dcr_stricts' has no match in constructor `NoDataConRep' of type `DataConRep'")
+  | DCR _ _ _ dcr_stricts _ => dcr_stricts
+  end.
+
+Definition dcr_wrap_id (arg_0__ : DataConRep) :=
+  match arg_0__ with
+  | NoDataConRep =>
+      GHC.Err.error (GHC.Base.hs_string__
+                     "Partial record selector: field `dcr_wrap_id' has no match in constructor `NoDataConRep' of type `DataConRep'")
+  | DCR dcr_wrap_id _ _ _ _ => dcr_wrap_id
+  end.
+
+Definition dcEqSpec (arg_0__ : DataCon) :=
+  let 'MkData _ _ _ _ _ _ _ dcEqSpec _ _ _ _ _ _ _ _ _ _ _ _ _ _ := arg_0__ in
+  dcEqSpec.
+
+Definition dcExTyVars (arg_0__ : DataCon) :=
+  let 'MkData _ _ _ _ _ dcExTyVars _ _ _ _ _ _ _ _ _ _ _ _ _ _ _ _ := arg_0__ in
+  dcExTyVars.
+
+Definition dcFields (arg_0__ : DataCon) :=
+  let 'MkData _ _ _ _ _ _ _ _ _ _ _ _ _ dcFields _ _ _ _ _ _ _ _ := arg_0__ in
+  dcFields.
+
+Definition dcInfix (arg_0__ : DataCon) :=
+  let 'MkData _ _ _ _ _ _ _ _ _ _ _ _ _ _ _ _ _ _ _ _ dcInfix _ := arg_0__ in
+  dcInfix.
+
+Definition dcName (arg_0__ : DataCon) :=
+  let 'MkData dcName _ _ _ _ _ _ _ _ _ _ _ _ _ _ _ _ _ _ _ _ _ := arg_0__ in
+  dcName.
+
+Definition dcOrigArgTys (arg_0__ : DataCon) :=
+  let 'MkData _ _ _ _ _ _ _ _ _ _ dcOrigArgTys _ _ _ _ _ _ _ _ _ _ _ := arg_0__ in
+  dcOrigArgTys.
+
+Definition dcOrigResTy (arg_0__ : DataCon) :=
+  let 'MkData _ _ _ _ _ _ _ _ _ _ _ dcOrigResTy _ _ _ _ _ _ _ _ _ _ := arg_0__ in
+  dcOrigResTy.
+
+Definition dcOtherTheta (arg_0__ : DataCon) :=
+  let 'MkData _ _ _ _ _ _ _ _ dcOtherTheta _ _ _ _ _ _ _ _ _ _ _ _ _ := arg_0__ in
+  dcOtherTheta.
+
+Definition dcPromoted (arg_0__ : DataCon) :=
+  let 'MkData _ _ _ _ _ _ _ _ _ _ _ _ _ _ _ _ _ _ _ _ _ dcPromoted := arg_0__ in
+  dcPromoted.
+
+Definition dcRep (arg_0__ : DataCon) :=
+  let 'MkData _ _ _ _ _ _ _ _ _ _ _ _ _ _ _ dcRep _ _ _ _ _ _ := arg_0__ in
+  dcRep.
+
+Definition dcRepArity (arg_0__ : DataCon) :=
+  let 'MkData _ _ _ _ _ _ _ _ _ _ _ _ _ _ _ _ dcRepArity _ _ _ _ _ := arg_0__ in
+  dcRepArity.
+
+Definition dcRepTyCon (arg_0__ : DataCon) :=
+  let 'MkData _ _ _ _ _ _ _ _ _ _ _ _ _ _ _ _ _ _ dcRepTyCon _ _ _ := arg_0__ in
+  dcRepTyCon.
+
+Definition dcRepType (arg_0__ : DataCon) :=
+  let 'MkData _ _ _ _ _ _ _ _ _ _ _ _ _ _ _ _ _ _ _ dcRepType _ _ := arg_0__ in
+  dcRepType.
+
+Definition dcSourceArity (arg_0__ : DataCon) :=
+  let 'MkData _ _ _ _ _ _ _ _ _ _ _ _ _ _ _ _ _ dcSourceArity _ _ _ _ :=
+    arg_0__ in
+  dcSourceArity.
+
+Definition dcSrcBangs (arg_0__ : DataCon) :=
+  let 'MkData _ _ _ _ _ _ _ _ _ _ _ _ dcSrcBangs _ _ _ _ _ _ _ _ _ := arg_0__ in
+  dcSrcBangs.
+
+Definition dcStupidTheta (arg_0__ : DataCon) :=
+  let 'MkData _ _ _ _ _ _ _ _ _ dcStupidTheta _ _ _ _ _ _ _ _ _ _ _ _ :=
+    arg_0__ in
+  dcStupidTheta.
+
+Definition dcTag (arg_0__ : DataCon) :=
+  let 'MkData _ _ dcTag _ _ _ _ _ _ _ _ _ _ _ _ _ _ _ _ _ _ _ := arg_0__ in
+  dcTag.
+
+Definition dcUnique (arg_0__ : DataCon) :=
+  let 'MkData _ dcUnique _ _ _ _ _ _ _ _ _ _ _ _ _ _ _ _ _ _ _ _ := arg_0__ in
+  dcUnique.
+
+Definition dcUnivTyVars (arg_0__ : DataCon) :=
+  let 'MkData _ _ _ _ dcUnivTyVars _ _ _ _ _ _ _ _ _ _ _ _ _ _ _ _ _ := arg_0__ in
+  dcUnivTyVars.
+
+Definition dcUserTyVarBinders (arg_0__ : DataCon) :=
+  let 'MkData _ _ _ _ _ _ dcUserTyVarBinders _ _ _ _ _ _ _ _ _ _ _ _ _ _ _ :=
+    arg_0__ in
+  dcUserTyVarBinders.
+
+Definition dcVanilla (arg_0__ : DataCon) :=
+  let 'MkData _ _ _ dcVanilla _ _ _ _ _ _ _ _ _ _ _ _ _ _ _ _ _ _ := arg_0__ in
+  dcVanilla.
+
+Definition dcWorkId (arg_0__ : DataCon) :=
+  let 'MkData _ _ _ _ _ _ _ _ _ _ _ _ _ _ dcWorkId _ _ _ _ _ _ _ := arg_0__ in
+  dcWorkId.
+(* Midamble *)
 
 Import FieldLabel.
 
-Parameter dataConSourceArity  : DataCon -> BasicTypes.Arity.
-Parameter dataConFieldLabels  : DataCon -> list FieldLabel.FieldLabel.
-Parameter dataConImplBangs    : DataCon -> HsImplBang.
-Parameter dataConName         : DataCon -> Name.Name.
-Parameter dataConTag          : DataCon -> BasicTypes.ConTag.
-
-Parameter dataConRepStrictness : DataCon -> SrcStrictness.
-(* Midamble *)
-
-
 Require GHC.Err.
-Instance Default_DataCon : GHC.Err.Default DataCon := {}.
+Instance Default__DataCon : GHC.Err.Default DataCon := {}.
 Admitted.
-
 
 Instance Uniqable_DataCon : Unique.Uniquable DataCon := {}.
 Admitted.
 
+(* Parameter dataConRepArgTys : DataCon -> list unit. *)
 
+(* Converted value declarations: *)
 
 Local Definition Eq___DataCon_op_zeze__ : DataCon -> DataCon -> bool :=
   fun a b => Unique.getUnique a GHC.Base.== Unique.getUnique b.
@@ -81,50 +258,718 @@ Local Definition Eq___DataCon_op_zeze__ : DataCon -> DataCon -> bool :=
 Local Definition Eq___DataCon_op_zsze__ : DataCon -> DataCon -> bool :=
   fun a b => Unique.getUnique a GHC.Base./= Unique.getUnique b.
 
-Program Instance Eq___DataCon : GHC.Base.Eq_ DataCon := fun _ k =>
-    k {|GHC.Base.op_zeze____ := Eq___DataCon_op_zeze__ ;
-      GHC.Base.op_zsze____ := Eq___DataCon_op_zsze__ |}.
+Program Instance Eq___DataCon : GHC.Base.Eq_ DataCon :=
+  fun _ k =>
+    k {| GHC.Base.op_zeze____ := Eq___DataCon_op_zeze__ ;
+         GHC.Base.op_zsze____ := Eq___DataCon_op_zsze__ |}.
 
+(* Translating `instance Uniquable__DataCon' failed: OOPS! Cannot find
+   information for class Qualified "Unique" "Uniquable" unsupported *)
+
+(* Translating `instance NamedThing__DataCon' failed: OOPS! Cannot find
+   information for class Qualified "Name" "NamedThing" unsupported *)
+
+(* Translating `instance Outputable__DataCon' failed: OOPS! Cannot find
+   information for class Qualified "Outputable" "Outputable" unsupported *)
+
+(* Translating `instance OutputableBndr__DataCon' failed: OOPS! Cannot find
+   information for class Qualified "Outputable" "OutputableBndr" unsupported *)
+
+(* Translating `instance Data__DataCon' failed: OOPS! Cannot find information
+   for class Qualified "Data.Data" "Data" unsupported *)
+
+(* Translating `instance Outputable__EqSpec' failed: OOPS! Cannot find
+   information for class Qualified "Outputable" "Outputable" unsupported *)
+
+(* Translating `instance Outputable__StrictnessMark' failed: OOPS! Cannot find
+   information for class Qualified "Outputable" "Outputable" unsupported *)
+
+(* Translating `instance Outputable__HsSrcBang' failed: OOPS! Cannot find
+   information for class Qualified "Outputable" "Outputable" unsupported *)
+
+(* Translating `instance Outputable__SrcUnpackedness' failed: OOPS! Cannot find
+   information for class Qualified "Outputable" "Outputable" unsupported *)
+
+(* Translating `instance Binary__SrcUnpackedness' failed: OOPS! Cannot find
+   information for class Qualified "Binary" "Binary" unsupported *)
+
+(* Translating `instance Outputable__SrcStrictness' failed: OOPS! Cannot find
+   information for class Qualified "Outputable" "Outputable" unsupported *)
+
+(* Translating `instance Binary__SrcStrictness' failed: OOPS! Cannot find
+   information for class Qualified "Binary" "Binary" unsupported *)
+
+(* Translating `instance Outputable__HsImplBang' failed: OOPS! Cannot find
+   information for class Qualified "Outputable" "Outputable" unsupported *)
+
+(* Translating `instance Data__HsSrcBang' failed: OOPS! Cannot find information
+   for class Qualified "Data.Data" "Data" unsupported *)
+
+(* Translating `instance Data__SrcUnpackedness' failed: OOPS! Cannot find
+   information for class Qualified "Data.Data" "Data" unsupported *)
 
 Local Definition Eq___SrcUnpackedness_op_zeze__
-    : SrcUnpackedness -> SrcUnpackedness -> bool :=
+   : SrcUnpackedness -> SrcUnpackedness -> bool :=
   fun arg_0__ arg_1__ =>
-    match arg_0__ , arg_1__ with
-      | SrcUnpack , SrcUnpack => true
-      | SrcNoUnpack , SrcNoUnpack => true
-      | NoSrcUnpack , NoSrcUnpack => true
-      | _ , _ => false
+    match arg_0__, arg_1__ with
+    | SrcUnpack, SrcUnpack => true
+    | SrcNoUnpack, SrcNoUnpack => true
+    | NoSrcUnpack, NoSrcUnpack => true
+    | _, _ => false
     end.
 
 Local Definition Eq___SrcUnpackedness_op_zsze__
-    : SrcUnpackedness -> SrcUnpackedness -> bool :=
-  fun a b => negb (Eq___SrcUnpackedness_op_zeze__ a b).
+   : SrcUnpackedness -> SrcUnpackedness -> bool :=
+  fun x y => negb (Eq___SrcUnpackedness_op_zeze__ x y).
 
-Program Instance Eq___SrcUnpackedness : GHC.Base.Eq_ SrcUnpackedness := fun _
-                                                                            k =>
-    k {|GHC.Base.op_zeze____ := Eq___SrcUnpackedness_op_zeze__ ;
-      GHC.Base.op_zsze____ := Eq___SrcUnpackedness_op_zsze__ |}.
+Program Instance Eq___SrcUnpackedness : GHC.Base.Eq_ SrcUnpackedness :=
+  fun _ k =>
+    k {| GHC.Base.op_zeze____ := Eq___SrcUnpackedness_op_zeze__ ;
+         GHC.Base.op_zsze____ := Eq___SrcUnpackedness_op_zsze__ |}.
 
-(* Translating `instance Data.Data.Data DataCon.SrcStrictness' failed: OOPS!
-   Cannot find information for class Qualified "Data.Data" "Data" unsupported *)
+(* Translating `instance Data__SrcStrictness' failed: OOPS! Cannot find
+   information for class Qualified "Data.Data" "Data" unsupported *)
 
 Local Definition Eq___SrcStrictness_op_zeze__
-    : SrcStrictness -> SrcStrictness -> bool :=
+   : SrcStrictness -> SrcStrictness -> bool :=
   fun arg_0__ arg_1__ =>
-    match arg_0__ , arg_1__ with
-      | SrcLazy , SrcLazy => true
-      | SrcStrict , SrcStrict => true
-      | NoSrcStrict , NoSrcStrict => true
-      | _ , _ => false
+    match arg_0__, arg_1__ with
+    | SrcLazy, SrcLazy => true
+    | SrcStrict, SrcStrict => true
+    | NoSrcStrict, NoSrcStrict => true
+    | _, _ => false
     end.
 
 Local Definition Eq___SrcStrictness_op_zsze__
-    : SrcStrictness -> SrcStrictness -> bool :=
-  fun a b => negb (Eq___SrcStrictness_op_zeze__ a b).
+   : SrcStrictness -> SrcStrictness -> bool :=
+  fun x y => negb (Eq___SrcStrictness_op_zeze__ x y).
 
-Program Instance Eq___SrcStrictness : GHC.Base.Eq_ SrcStrictness := fun _ k =>
-    k {|GHC.Base.op_zeze____ := Eq___SrcStrictness_op_zeze__ ;
-      GHC.Base.op_zsze____ := Eq___SrcStrictness_op_zsze__ |}.
+Program Instance Eq___SrcStrictness : GHC.Base.Eq_ SrcStrictness :=
+  fun _ k =>
+    k {| GHC.Base.op_zeze____ := Eq___SrcStrictness_op_zeze__ ;
+         GHC.Base.op_zsze____ := Eq___SrcStrictness_op_zsze__ |}.
 
-(* Translating `instance Data.Data.Data DataCon.HsImplBang' failed: OOPS! Cannot
-   find information for class Qualified "Data.Data" "Data" unsupported *)
+(* Translating `instance Data__HsImplBang' failed: OOPS! Cannot find information
+   for class Qualified "Data.Data" "Data" unsupported *)
+
+(*
+Definition buildAlgTyCon
+   : Name.Name ->
+     list Var.TyVar ->
+     list CoAxiom.Role ->
+     option unit ->
+     unit -> TyCon.AlgTyConRhs -> bool -> unut -> unit := tt.
+  fun tc_name ktvs roles cType stupid_theta rhs gadt_syn parent => tt.
+    let binders := Type.mkTyConBindersPreferAnon ktvs TysWiredIn.liftedTypeKind in
+    TyCon.mkAlgTyCon tc_name binders TysWiredIn.liftedTypeKind roles cType
+    stupid_theta rhs parent gadt_syn. 
+
+Definition buildSynTyCon
+   : Name.Name ->
+     list TyCon.TyConBinder -> unit -> list CoAxiom.Role -> unit -> unit :=
+  fun name binders res_kind roles rhs =>
+    let is_fam_free := Type.isFamFreeTy rhs in
+    let is_tau := Type.isTauTy rhs in
+    TyCon.mkSynonymTyCon name binders res_kind roles rhs is_tau is_fam_free.
+*)
+
+Definition classDataCon : Class.Class -> DataCon :=
+  fun clas =>
+    match TyCon.tyConDataCons (Class.classTyCon clas) with
+    | cons dict_constr no_more =>
+        if andb Util.debugIsOn (negb (Data.Foldable.null no_more)) : bool
+        then (Panic.assertPanic (GHC.Base.hs_string__
+                                 "ghc/compiler/basicTypes/DataCon.hs") #1346)
+        else dict_constr
+    | nil => Panic.panic (GHC.Base.hs_string__ "classDataCon")
+    end.
+
+Definition dataConBoxer : DataCon -> option unit :=
+  fun arg_0__ =>
+    match arg_0__ with
+    | MkData _ _ _ _ _ _ _ _ _ _ _ _ _ _ _ (DCR _ boxer _ _ _) _ _ _ _ _ _ =>
+        Some boxer
+    | _ => None
+    end.
+
+Definition dataConExTyVars : DataCon -> list Var.TyVar :=
+  fun arg_0__ =>
+    let 'MkData _ _ _ _ _ tvbs _ _ _ _ _ _ _ _ _ _ _ _ _ _ _ _ := arg_0__ in
+    tvbs.
+
+Definition dataConFieldLabels : DataCon -> list FieldLabel.FieldLabel :=
+  dcFields.
+
+Definition dataConFieldType_maybe
+   : DataCon ->
+     FieldLabel.FieldLabelString -> option (FieldLabel.FieldLabel * unit)%type :=
+  fun con label =>
+    Data.Foldable.find ((fun arg_0__ => arg_0__ GHC.Base.== label) GHC.Base.∘
+                        (FieldLabel.flLabel GHC.Base.∘ Data.Tuple.fst)) (GHC.List.zip (dcFields con)
+                                                                                      (dcOrigArgTys con)).
+
+Definition dataConFieldType : DataCon -> FieldLabel.FieldLabelString -> unit :=
+  fun con label =>
+    match dataConFieldType_maybe con label with
+    | Some (pair _ ty) => ty
+    | None =>
+        Panic.panicStr (GHC.Base.hs_string__ "dataConFieldType") (GHC.Base.mappend
+                                                                  (Panic.noString con) (Panic.noString label))
+    end.
+
+Definition dataConFullSig
+   : DataCon ->
+     (list Var.TyVar * list Var.TyVar * list EqSpec * unit * list unit *
+      unit)%type :=
+  fun arg_0__ =>
+    let 'MkData _ _ _ _ univ_tvs ex_tvs _ eq_spec theta _ arg_tys res_ty _ _ _ _ _ _
+       _ _ _ _ := arg_0__ in
+    pair (pair (pair (pair (pair univ_tvs ex_tvs) eq_spec) theta) arg_tys) res_ty.
+
+Definition dataConImplBangs : DataCon -> list HsImplBang :=
+  fun dc =>
+    match dcRep dc with
+    | NoDataConRep => GHC.List.replicate (dcSourceArity dc) HsLazy
+    | DCR _ _ _ _ bangs => bangs
+    end.
+
+Definition dataConImplicitTyThings : DataCon -> list unit :=
+  fun arg_0__ =>
+    let 'MkData _ _ _ _ _ _ _ _ _ _ _ _ _ _ work rep _ _ _ _ _ _ := arg_0__ in
+    let wrap_ids :=
+      match rep with
+      | NoDataConRep => nil
+      | DCR wrap _ _ _ _ => cons (TyCoRep.AnId wrap) nil
+      end in
+    Coq.Init.Datatypes.app (cons (TyCoRep.AnId work) nil) wrap_ids.
+
+Definition dataConInstOrigArgTys : DataCon -> list unit -> list unit :=
+  fun arg_0__ arg_1__ =>
+    match arg_0__, arg_1__ with
+    | (MkData _ _ _ _ univ_tvs ex_tvs _ _ _ _ arg_tys _ _ _ _ _ _ _ _ _ _ _ as dc)
+    , inst_tys =>
+        let tyvars := Coq.Init.Datatypes.app univ_tvs ex_tvs in
+        if andb Util.debugIsOn (negb (Util.equalLength tyvars inst_tys)) : bool
+        then (Outputable.assertPprPanic (GHC.Base.hs_string__
+                                         "ghc/compiler/basicTypes/DataCon.hs") #1274 ((GHC.Base.mappend (id
+                                                                                                         (GHC.Base.hs_string__
+                                                                                                          "dataConInstOrigArgTys"))
+                                                                                                        (Panic.noString
+                                                                                                         dc)
+                                                                                       Outputable.$$
+                                                                                       Panic.noString tyvars)
+                                                                                      Outputable.$$
+                                                                                      Panic.noString inst_tys))
+        else GHC.Base.map (TyCoRep.substTyWith tyvars inst_tys) arg_tys
+    end.
+
+Definition dataConIsInfix : DataCon -> bool :=
+  dcInfix.
+
+Definition dataConName : DataCon -> Name.Name :=
+  dcName.
+
+Definition dataConOrigArgTys : DataCon -> list unit :=
+  fun dc => dcOrigArgTys dc.
+
+Definition dataConOrigResTy : DataCon -> unit :=
+  fun dc => dcOrigResTy dc.
+
+Definition dataConOrigTyCon : DataCon -> unit :=
+  fun dc =>
+    match TyCon.tyConFamInst_maybe (dcRepTyCon dc) with
+    | Some (pair tc _) => tc
+    | _ => dcRepTyCon dc
+    end.
+
+Definition dataConRepArgTys : DataCon -> list unit :=
+  fun arg_0__ =>
+    let 'MkData _ _ _ _ _ _ _ eq_spec theta _ orig_arg_tys _ _ _ _ rep _ _ _ _ _
+       _ := arg_0__ in
+    match rep with
+    | NoDataConRep =>
+        if andb Util.debugIsOn (negb (Data.Foldable.null eq_spec)) : bool
+        then (Panic.assertPanic (GHC.Base.hs_string__
+                                 "ghc/compiler/basicTypes/DataCon.hs") #1293)
+        else Coq.Init.Datatypes.app theta orig_arg_tys
+    | DCR _ _ arg_tys _ _ => arg_tys
+    end.
+
+Definition dataConRepStrictness : DataCon -> list StrictnessMark :=
+  fun dc =>
+    match dcRep dc with
+    | NoDataConRep =>
+        Coq.Lists.List.flat_map (fun _ => cons NotMarkedStrict nil) (dataConRepArgTys
+                                 dc)
+    | DCR _ _ _ strs _ => strs
+    end.
+
+Definition dataConInstArgTys : DataCon -> list unit -> list unit :=
+  fun arg_0__ arg_1__ =>
+    match arg_0__, arg_1__ with
+    | (MkData _ _ _ _ univ_tvs ex_tvs _ _ _ _ _ _ _ _ _ _ _ _ _ _ _ _ as dc)
+    , inst_tys =>
+        if andb Util.debugIsOn (negb (Util.equalLength univ_tvs inst_tys)) : bool
+        then (Outputable.assertPprPanic (GHC.Base.hs_string__
+                                         "ghc/compiler/basicTypes/DataCon.hs") #1257 ((GHC.Base.mappend (id
+                                                                                                         (GHC.Base.hs_string__
+                                                                                                          "dataConInstArgTys"))
+                                                                                                        (Panic.noString
+                                                                                                         dc)
+                                                                                       Outputable.$$
+                                                                                       Panic.noString univ_tvs)
+                                                                                      Outputable.$$
+                                                                                      Panic.noString inst_tys))
+        else if andb Util.debugIsOn (negb (Data.Foldable.null ex_tvs)) : bool
+             then (Outputable.assertPprPanic (GHC.Base.hs_string__
+                                              "ghc/compiler/basicTypes/DataCon.hs") #1258 (Panic.noString dc))
+             else GHC.Base.map (TyCoRep.substTyWith univ_tvs inst_tys) (dataConRepArgTys dc)
+    end.
+
+Definition splitDataProductType_maybe
+   : unit -> option (unit * list unit * DataCon * list unit)%type :=
+  fun ty =>
+    match Type.splitTyConApp_maybe ty with
+    | Some (pair tycon ty_args) =>
+        match TyCon.isDataProductTyCon_maybe tycon with
+        | Some con =>
+            Some (pair (pair (pair tycon ty_args) con) (dataConInstArgTys con ty_args))
+        | _ => None
+        end
+    | _ => None
+    end.
+
+Definition dataConRepArity : DataCon -> BasicTypes.Arity :=
+  fun arg_0__ =>
+    let 'MkData _ _ _ _ _ _ _ _ _ _ _ _ _ _ _ _ arity _ _ _ _ _ := arg_0__ in
+    arity.
+
+Definition isNullaryRepDataCon : DataCon -> bool :=
+  fun dc => dataConRepArity dc GHC.Base.== #0.
+
+Definition dataConRepType : DataCon -> unit :=
+  dcRepType.
+
+Definition dataConSourceArity : DataCon -> BasicTypes.Arity :=
+  fun arg_0__ =>
+    let 'MkData _ _ _ _ _ _ _ _ _ _ _ _ _ _ _ _ _ arity _ _ _ _ := arg_0__ in
+    arity.
+
+Definition isNullarySrcDataCon : DataCon -> bool :=
+  fun dc => dataConSourceArity dc GHC.Base.== #0.
+
+Definition dataConSrcBangs : DataCon -> list HsSrcBang :=
+  dcSrcBangs.
+
+Definition dataConStupidTheta : DataCon -> unit :=
+  fun dc => dcStupidTheta dc.
+
+Definition dataConTag : DataCon -> BasicTypes.ConTag :=
+  dcTag.
+
+Definition dataConTagZ : DataCon -> BasicTypes.ConTagZ :=
+  fun con => dataConTag con GHC.Num.- BasicTypes.fIRST_TAG.
+
+Definition dataConTyCon : DataCon -> unit :=
+  dcRepTyCon.
+
+Definition specialPromotedDc : DataCon -> bool :=
+  TyCon.isKindTyCon GHC.Base.∘ dataConTyCon.
+
+Definition dataConUnivAndExTyVars : DataCon -> list Var.TyVar :=
+  fun arg_0__ =>
+    let 'MkData _ _ _ _ univ_tvs ex_tvs _ _ _ _ _ _ _ _ _ _ _ _ _ _ _ _ :=
+      arg_0__ in
+    Coq.Init.Datatypes.app univ_tvs ex_tvs.
+
+Definition dataConUnivTyVars : DataCon -> list Var.TyVar :=
+  fun arg_0__ =>
+    let 'MkData _ _ _ _ tvbs _ _ _ _ _ _ _ _ _ _ _ _ _ _ _ _ _ := arg_0__ in
+    tvbs.
+
+Definition dataConUserTyVarBinders : DataCon -> list Var.TyVarBinder :=
+  dcUserTyVarBinders.
+
+Definition dataConUserTyVars : DataCon -> list Var.TyVar :=
+  fun arg_0__ =>
+    let 'MkData _ _ _ _ _ _ tvbs _ _ _ _ _ _ _ _ _ _ _ _ _ _ _ := arg_0__ in
+    Var.binderVars tvbs.
+
+Definition dataConUserType : DataCon -> unit :=
+  fun arg_0__ =>
+    let 'MkData _ _ _ _ _ _ user_tvbs _ theta _ arg_tys res_ty _ _ _ _ _ _ _ _ _
+       _ := arg_0__ in
+    TyCoRep.mkForAllTys user_tvbs (TyCoRep.mkFunTys theta (TyCoRep.mkFunTys arg_tys
+                                                                            res_ty)).
+
+Definition dataConWorkId : DataCon -> Var.Id :=
+  fun dc => dcWorkId dc.
+
+Definition dataConWrapId : DataCon -> Var.Id :=
+  fun dc =>
+    match dcRep dc with
+    | NoDataConRep => dcWorkId dc
+    | DCR wrap_id _ _ _ _ => wrap_id
+    end.
+
+Definition dataConWrapId_maybe : DataCon -> option Var.Id :=
+  fun dc =>
+    match dcRep dc with
+    | NoDataConRep => None
+    | DCR wrap_id _ _ _ _ => Some wrap_id
+    end.
+
+Definition eqHsBang : HsImplBang -> HsImplBang -> bool :=
+  fun arg_0__ arg_1__ =>
+    match arg_0__, arg_1__ with
+    | HsLazy, HsLazy => true
+    | HsStrict, HsStrict => true
+    | HsUnpack None, HsUnpack None => true
+    | HsUnpack (Some c1), HsUnpack (Some c2) =>
+        Type.eqType (Coercion.coercionType c1) (Coercion.coercionType c2)
+    | _, _ => false
+    end.
+
+Definition eqSpecPair : EqSpec -> (Var.TyVar * unit)%type :=
+  fun arg_0__ => let 'Mk_EqSpec tv ty := arg_0__ in pair tv ty.
+
+Definition eqSpecPreds : list EqSpec -> unit :=
+  fun spec =>
+    let cont_0__ arg_1__ :=
+      let 'Mk_EqSpec tv ty := arg_1__ in
+      cons (Type.mkPrimEqPred (TyCoRep.mkTyVarTy tv) ty) nil in
+    Coq.Lists.List.flat_map cont_0__ spec.
+
+Definition dataConTheta : DataCon -> unit :=
+  fun arg_0__ =>
+    let 'MkData _ _ _ _ _ _ _ eq_spec theta _ _ _ _ _ _ _ _ _ _ _ _ _ := arg_0__ in
+    Coq.Init.Datatypes.app (eqSpecPreds eq_spec) theta.
+
+Definition dataConSig
+   : DataCon -> (list Var.TyVar * unit * list unit * unit)%type :=
+  fun arg_0__ =>
+    let '(MkData _ _ _ _ _ _ _ _ _ _ arg_tys res_ty _ _ _ _ _ _ _ _ _ _ as con) :=
+      arg_0__ in
+    pair (pair (pair (dataConUnivAndExTyVars con) (dataConTheta con)) arg_tys)
+         res_ty.
+
+Definition dataConInstSig
+   : DataCon -> list unit -> (list Var.TyVar * unit * list unit)%type :=
+  fun arg_0__ arg_1__ =>
+    match arg_0__, arg_1__ with
+    | MkData _ _ _ _ univ_tvs ex_tvs _ eq_spec theta _ arg_tys _ _ _ _ _ _ _ _ _ _ _
+    , univ_tys =>
+        let univ_subst := TyCoRep.zipTvSubst univ_tvs univ_tys in
+        let 'pair subst ex_tvs' := Data.Traversable.mapAccumL TyCoRep.substTyVarBndr
+                                     univ_subst ex_tvs in
+        pair (pair ex_tvs' (TyCoRep.substTheta subst (Coq.Init.Datatypes.app
+                                                      (eqSpecPreds eq_spec) theta))) (TyCoRep.substTys subst arg_tys)
+    end.
+
+Definition dataConCannotMatch : list unit -> DataCon -> bool :=
+  fun tys con =>
+    let predEqs :=
+      fun pred =>
+        match Type.classifyPredType pred with
+        | Type.EqPred Type.NomEq ty1 ty2 => cons (pair ty1 ty2) nil
+        | Type.ClassPred eq (cons _ (cons ty1 (cons ty2 nil))) =>
+            if Unique.hasKey eq PrelNames.eqTyConKey : bool
+            then cons (pair ty1 ty2) nil else
+            nil
+        end in
+    let 'pair (pair _ inst_theta) _ := dataConInstSig con tys in
+    if Data.Foldable.null inst_theta : bool then false else
+    if Data.Foldable.all Type.isTyVarTy tys : bool then false else
+    Unify.typesCantMatch (Data.Foldable.concatMap predEqs inst_theta).
+
+Definition eqSpecTyVar : EqSpec -> Var.TyVar :=
+  fun arg_0__ => let 'Mk_EqSpec tv _ := arg_0__ in tv.
+
+Definition filterEqSpec : list EqSpec -> list Var.TyVar -> list Var.TyVar :=
+  fun eq_spec =>
+    let not_in_eq_spec :=
+      fun var =>
+        Data.Foldable.all (negb GHC.Base.∘
+                           ((fun arg_0__ => arg_0__ GHC.Base.== var) GHC.Base.∘ eqSpecTyVar)) eq_spec in
+    GHC.List.filter not_in_eq_spec.
+
+Definition dataConUserTyVarsArePermuted : DataCon -> bool :=
+  fun arg_0__ =>
+    let 'MkData _ _ _ _ univ_tvs ex_tvs user_tvbs eq_spec _ _ _ _ _ _ _ _ _ _ _ _ _
+       _ := arg_0__ in
+    (Coq.Init.Datatypes.app (filterEqSpec eq_spec univ_tvs) ex_tvs) GHC.Base./=
+    Var.binderVars user_tvbs.
+
+Definition eqSpecType : EqSpec -> unit :=
+  fun arg_0__ => let 'Mk_EqSpec _ ty := arg_0__ in ty.
+
+Definition freshNames : list Name.Name -> list Name.Name :=
+  fun avoids =>
+    let avoid_occs : OccName.OccSet :=
+      OccName.mkOccSet (GHC.Base.map Name.getOccName avoids) in
+    let avoid_uniqs : UniqSet.UniqSet Unique.Unique :=
+      UniqSet.mkUniqSet (GHC.Base.map Unique.getUnique avoids) in
+    Coq.Lists.List.flat_map (fun n =>
+                               let occ :=
+                                 OccName.mkTyVarOccFS (FastString.mkFastString (cons (GHC.Char.hs_char__ "x")
+                                                                                     (GHC.Show.show n))) in
+                               let uniq := Unique.mkAlphaTyVarUnique n in
+                               if negb (UniqSet.elementOfUniqSet uniq avoid_uniqs) : bool
+                               then if negb (OccName.elemOccSet occ avoid_occs) : bool
+                                    then cons (Name.mkSystemName uniq occ) nil else
+                                    nil else
+                               nil) (enumFrom #0).
+
+Definition mkCleanAnonTyConBinders
+   : list TyCon.TyConBinder -> list unit -> list TyCon.TyConBinder :=
+  fun tc_bndrs tys =>
+    let fresh_names :=
+      freshNames (GHC.Base.map Name.getName (Var.binderVars tc_bndrs)) in
+    let cont_1__ arg_2__ :=
+      let 'pair name ty := arg_2__ in
+      cons (TyCon.mkAnonTyConBinder (Var.mkTyVar name ty)) nil in
+    Coq.Lists.List.flat_map cont_1__ (GHC.List.zip fresh_names tys).
+
+Definition mkDataCon
+   : Name.Name ->
+     bool ->
+     TyCon.TyConRepName ->
+     list HsSrcBang ->
+     list FieldLabel.FieldLabel ->
+     list Var.TyVar ->
+     list Var.TyVar ->
+     list Var.TyVarBinder ->
+     list EqSpec ->
+     unit ->
+     list unit ->
+     unit ->
+     TyCon.RuntimeRepInfo -> unit -> unit -> Var.Id -> DataConRep -> DataCon :=
+  fun name
+  declared_infix
+  prom_info
+  arg_stricts
+  fields
+  univ_tvs
+  ex_tvs
+  user_tvbs
+  eq_spec
+  theta
+  orig_arg_tys
+  orig_res_ty
+  rep_info
+  rep_tycon
+  stupid_theta
+  work_id
+  rep =>
+    let roles :=
+      Coq.Init.Datatypes.app (GHC.Base.map (GHC.Base.const CoAxiom.Nominal)
+                              (Coq.Init.Datatypes.app univ_tvs ex_tvs)) (GHC.Base.map (GHC.Base.const
+                                                                                       CoAxiom.Representational)
+                              orig_arg_tys) in
+    let prom_res_kind := orig_res_ty in
+    let user_tvbs_invariant :=
+      Data.Set.Internal.fromList (Coq.Init.Datatypes.app (filterEqSpec eq_spec
+                                                          univ_tvs) ex_tvs) GHC.Base.==
+      Data.Set.Internal.fromList (Var.binderVars user_tvbs) in
+    let user_tvbs' :=
+      if andb Util.debugIsOn (negb (user_tvbs_invariant)) : bool
+      then (Outputable.assertPprPanic (GHC.Base.hs_string__
+                                       "ghc/compiler/basicTypes/DataCon.hs") #897 ((Panic.noString univ_tvs
+                                                                                    Outputable.$$
+                                                                                    Panic.noString ex_tvs) Outputable.$$
+                                                                                   Panic.noString user_tvbs))
+      else user_tvbs in
+    let prom_tv_bndrs :=
+      let cont_3__ arg_4__ :=
+        match arg_4__ with
+        | Var.TvBndr tv vis => cons (TyCon.mkNamedTyConBinder vis tv) nil
+        | _ => nil
+        end in
+      Coq.Lists.List.flat_map cont_3__ user_tvbs' in
+    let prom_arg_bndrs :=
+      mkCleanAnonTyConBinders prom_tv_bndrs (Coq.Init.Datatypes.app theta
+                                                                    orig_arg_tys) in
+    let is_vanilla :=
+      andb (Data.Foldable.null ex_tvs) (andb (Data.Foldable.null eq_spec)
+                                             (Data.Foldable.null theta)) in
+    let con :=
+      MkData name (Name.nameUnique name) tag is_vanilla univ_tvs ex_tvs user_tvbs'
+             eq_spec theta stupid_theta orig_arg_tys orig_res_ty arg_stricts fields work_id
+             rep (Data.Foldable.length rep_arg_tys) (Data.Foldable.length orig_arg_tys)
+             rep_tycon rep_ty declared_infix promoted in
+    let tag :=
+      ListSetOps.assoc (GHC.Base.hs_string__ "mkDataCon") (GHC.List.zip
+                                                           (TyCon.tyConDataCons rep_tycon) (enumFrom
+                                                            BasicTypes.fIRST_TAG)) con in
+    let rep_arg_tys := dataConRepArgTys con in
+    let rep_ty :=
+      match rep with
+      | NoDataConRep => dataConUserType con
+      | DCR _ _ _ _ _ =>
+          Type.mkInvForAllTys univ_tvs (Type.mkInvForAllTys ex_tvs (TyCoRep.mkFunTys
+                                                             rep_arg_tys (Type.mkTyConApp rep_tycon (TyCoRep.mkTyVarTys
+                                                                                           univ_tvs))))
+      end in
+    let promoted :=
+      TyCon.mkPromotedDataCon con name prom_info (Coq.Init.Datatypes.app prom_tv_bndrs
+                                                                         prom_arg_bndrs) prom_res_kind roles rep_info in
+    con.
+
+Definition isBanged : HsImplBang -> bool :=
+  fun arg_0__ =>
+    match arg_0__ with
+    | HsUnpack _ => true
+    | HsStrict => true
+    | HsLazy => false
+    end.
+
+Definition isLegacyPromotableTyCon : unit -> bool :=
+  fun tc =>
+    orb (TyCon.isVanillaAlgTyCon tc) (orb (TyCon.isFunTyCon tc) (TyCon.isKindTyCon
+                                           tc)).
+
+Definition isMarkedStrict : StrictnessMark -> bool :=
+  fun arg_0__ => match arg_0__ with | NotMarkedStrict => false | _ => true end.
+
+Definition isSrcStrict : SrcStrictness -> bool :=
+  fun arg_0__ => match arg_0__ with | SrcStrict => true | _ => false end.
+
+Definition isSrcUnpacked : SrcUnpackedness -> bool :=
+  fun arg_0__ => match arg_0__ with | SrcUnpack => true | _ => false end.
+
+Definition isTupleDataCon : DataCon -> bool :=
+  fun arg_0__ =>
+    let 'MkData _ _ _ _ _ _ _ _ _ _ _ _ _ _ _ _ _ _ tc _ _ _ := arg_0__ in
+    TyCon.isTupleTyCon tc.
+
+Definition isUnboxedSumCon : DataCon -> bool :=
+  fun arg_0__ =>
+    let 'MkData _ _ _ _ _ _ _ _ _ _ _ _ _ _ _ _ _ _ tc _ _ _ := arg_0__ in
+    TyCon.isUnboxedSumTyCon tc.
+
+Definition isUnboxedTupleCon : DataCon -> bool :=
+  fun arg_0__ =>
+    let 'MkData _ _ _ _ _ _ _ _ _ _ _ _ _ _ _ _ _ _ tc _ _ _ := arg_0__ in
+    TyCon.isUnboxedTupleTyCon tc.
+
+Definition isVanillaDataCon : DataCon -> bool :=
+  fun dc => dcVanilla dc.
+
+Definition mkEqSpec : Var.TyVar -> unit -> EqSpec :=
+  fun tv ty => Mk_EqSpec tv ty.
+
+Definition dataConEqSpec : DataCon -> list EqSpec :=
+  fun arg_0__ =>
+    let 'MkData _ _ _ _ _ _ _ eq_spec theta _ _ _ _ _ _ _ _ _ _ _ _ _ := arg_0__ in
+    Coq.Init.Datatypes.app eq_spec (Coq.Init.Datatypes.app (let cont_1__ arg_2__ :=
+                                                              match arg_2__ with
+                                                              | Some (pair tc (cons _k1 (cons _k2 (cons ty1 (cons ty2
+                                                                   nil))))) =>
+                                                                  if Unique.hasKey tc PrelNames.heqTyConKey : bool
+                                                                  then Coq.Lists.List.flat_map (fun spec =>
+                                                                                                  cons spec nil)
+                                                                                               (match pair
+                                                                                                        (Type.getTyVar_maybe
+                                                                                                         ty1)
+                                                                                                        (Type.getTyVar_maybe
+                                                                                                         ty2) with
+                                                                                                | pair (Some tv1) _ =>
+                                                                                                    cons (mkEqSpec tv1
+                                                                                                          ty2) nil
+                                                                                                | pair _ (Some tv2) =>
+                                                                                                    cons (mkEqSpec tv2
+                                                                                                          ty1) nil
+                                                                                                | _ => nil
+                                                                                                end) else
+                                                                  nil
+                                                              | _ => nil
+                                                              end in
+                                                            Coq.Lists.List.flat_map cont_1__ (GHC.Base.map
+                                                                                     Type.splitTyConApp_maybe theta))
+                                                           (let cont_7__ arg_8__ :=
+                                                              match arg_8__ with
+                                                              | Some (pair tc (cons _k (cons ty1 (cons ty2 nil)))) =>
+                                                                  if Unique.hasKey tc PrelNames.eqTyConKey : bool
+                                                                  then Coq.Lists.List.flat_map (fun spec =>
+                                                                                                  cons spec nil)
+                                                                                               (match pair
+                                                                                                        (Type.getTyVar_maybe
+                                                                                                         ty1)
+                                                                                                        (Type.getTyVar_maybe
+                                                                                                         ty2) with
+                                                                                                | pair (Some tv1) _ =>
+                                                                                                    cons (mkEqSpec tv1
+                                                                                                          ty2) nil
+                                                                                                | pair _ (Some tv2) =>
+                                                                                                    cons (mkEqSpec tv2
+                                                                                                          ty1) nil
+                                                                                                | _ => nil
+                                                                                                end) else
+                                                                  nil
+                                                              | _ => nil
+                                                              end in
+                                                            Coq.Lists.List.flat_map cont_7__ (GHC.Base.map
+                                                                                     Type.splitTyConApp_maybe theta))).
+
+Definition isLegacyPromotableDataCon : DataCon -> bool :=
+  fun dc =>
+    andb (Data.Foldable.null (dataConEqSpec dc)) (andb (Data.Foldable.null
+                                                        (dataConTheta dc)) (andb (negb (TyCon.isFamInstTyCon
+                                                                                        (dataConTyCon dc)))
+                                                                                 (UniqSet.uniqSetAll
+                                                                                  isLegacyPromotableTyCon
+                                                                                  (Type.tyConsOfType (dataConUserType
+                                                                                                      dc))))).
+
+Definition promoteDataCon : DataCon -> unit :=
+  fun arg_0__ =>
+    let 'MkData _ _ _ _ _ _ _ _ _ _ _ _ _ _ _ _ _ _ _ _ _ tc := arg_0__ in
+    tc.
+
+Definition substEqSpec : TyCoRep.TCvSubst -> EqSpec -> EqSpec :=
+  fun arg_0__ arg_1__ =>
+    match arg_0__, arg_1__ with
+    | subst, Mk_EqSpec tv ty =>
+        let tv' :=
+          Type.getTyVar (GHC.Base.hs_string__ "substEqSpec") (TyCoRep.substTyVar subst
+                                                              tv) in
+        Mk_EqSpec tv' (TyCoRep.substTy subst ty)
+    end.
+
+(* External variables:
+     None Some andb bool cons enumFrom false id list negb nil op_zt__ option orb pair
+     promoted rep_arg_tys rep_ty tag true unit BasicTypes.Arity BasicTypes.ConTag
+     BasicTypes.ConTagZ BasicTypes.SourceText BasicTypes.fIRST_TAG Class.Class
+     Class.classTyCon CoAxiom.Nominal CoAxiom.Representational CoAxiom.Role
+     Coercion.coercionType Coq.Init.Datatypes.app Coq.Lists.List.flat_map
+     Data.Foldable.all Data.Foldable.concatMap Data.Foldable.find
+     Data.Foldable.length Data.Foldable.null Data.Set.Internal.fromList
+     Data.Traversable.mapAccumL Data.Tuple.fst FastString.mkFastString
+     FieldLabel.FieldLabel FieldLabel.FieldLabelString FieldLabel.flLabel
+     ForeignCall.CType GHC.Base.Eq_ GHC.Base.const GHC.Base.map GHC.Base.mappend
+     GHC.Base.op_z2218U__ GHC.Base.op_zeze__ GHC.Base.op_zsze__ GHC.Err.Build_Default
+     GHC.Err.Default GHC.Err.error GHC.List.filter GHC.List.replicate GHC.List.zip
+     GHC.Num.fromInteger GHC.Num.op_zm__ GHC.Show.show ListSetOps.assoc Name.Name
+     Name.getName Name.getOccName Name.mkSystemName Name.nameUnique OccName.OccSet
+     OccName.elemOccSet OccName.mkOccSet OccName.mkTyVarOccFS
+     Outputable.assertPprPanic Outputable.op_zdzd__ Panic.assertPanic Panic.noString
+     Panic.panic Panic.panicStr PrelNames.eqTyConKey PrelNames.heqTyConKey
+     TyCoRep.AnId TyCoRep.TCvSubst TyCoRep.mkForAllTys TyCoRep.mkFunTys
+     TyCoRep.mkTyVarTy TyCoRep.mkTyVarTys TyCoRep.substTheta TyCoRep.substTy
+     TyCoRep.substTyVar TyCoRep.substTyVarBndr TyCoRep.substTyWith TyCoRep.substTys
+     TyCoRep.zipTvSubst TyCon.AlgTyConFlav TyCon.AlgTyConRhs TyCon.RuntimeRepInfo
+     TyCon.TyConBinder TyCon.TyConRepName TyCon.isDataProductTyCon_maybe
+     TyCon.isFamInstTyCon TyCon.isFunTyCon TyCon.isKindTyCon TyCon.isTupleTyCon
+     TyCon.isUnboxedSumTyCon TyCon.isUnboxedTupleTyCon TyCon.isVanillaAlgTyCon
+     TyCon.mkAlgTyCon TyCon.mkAnonTyConBinder TyCon.mkNamedTyConBinder
+     TyCon.mkPromotedDataCon TyCon.mkSynonymTyCon TyCon.tyConDataCons
+     TyCon.tyConFamInst_maybe Type.ClassPred Type.EqPred Type.NomEq
+     Type.classifyPredType Type.eqType Type.getTyVar Type.getTyVar_maybe
+     Type.isFamFreeTy Type.isTauTy Type.isTyVarTy Type.mkInvForAllTys
+     Type.mkPrimEqPred Type.mkTyConApp Type.mkTyConBindersPreferAnon
+     Type.splitTyConApp_maybe Type.tyConsOfType TysWiredIn.liftedTypeKind
+     Unify.typesCantMatch UniqSet.UniqSet UniqSet.elementOfUniqSet UniqSet.mkUniqSet
+     UniqSet.uniqSetAll Unique.Unique Unique.getUnique Unique.hasKey
+     Unique.mkAlphaTyVarUnique Util.debugIsOn Util.equalLength Var.Id Var.TvBndr
+     Var.TyVar Var.TyVarBinder Var.binderVars Var.mkTyVar
+*)
