examples/ghc/lib/CoreSubst.v
@@ -12,26 +12,28 @@ Require Coq.Program.Wf.
 
 (* Preamble *)
 
-Require Import Core.
+
 
 (* Converted imports: *)
 
 Require CoreSyn.
-Require CoreType.
 Require IdInfo.
 Require Name.
 Require UniqSupply.
 Require Unique.
+Require Var.
+Require VarEnv.
+Require VarSet.
 
 (* Converted type declarations: *)
 
 Definition IdSubstEnv :=
-  (CoreType.IdEnv CoreSyn.CoreExpr)%type.
+  (VarEnv.IdEnv CoreSyn.CoreExpr)%type.
 
 Inductive Subst : Type
   := Mk_Subst
-   : CoreType.InScopeSet ->
-     IdSubstEnv -> CoreType.TvSubstEnv -> CoreType.CvSubstEnv -> Subst.
+   : VarEnv.InScopeSet ->
+     IdSubstEnv -> TyCoRep.TvSubstEnv -> TyCoRep.CvSubstEnv -> Subst.
 (* Converted value declarations: *)
 
 Axiom substUnfoldingSC : Subst -> CoreSyn.Unfolding -> CoreSyn.Unfolding.
@@ -47,132 +49,123 @@ Axiom deShadowBinds : CoreSyn.CoreProgram -> CoreSyn.CoreProgram.
 
 Axiom emptySubst : Subst.
 
-Axiom mkEmptySubst : CoreType.InScopeSet -> Subst.
+Axiom mkEmptySubst : VarEnv.InScopeSet -> Subst.
 
-Axiom mkSubst : CoreType.InScopeSet ->
-                CoreType.TvSubstEnv -> CoreType.CvSubstEnv -> IdSubstEnv -> Subst.
+Axiom mkSubst : VarEnv.InScopeSet ->
+                TyCoRep.TvSubstEnv -> TyCoRep.CvSubstEnv -> IdSubstEnv -> Subst.
 
-Axiom substInScope : Subst -> CoreType.InScopeSet.
+Axiom substInScope : Subst -> VarEnv.InScopeSet.
 
 Axiom zapSubstEnv : Subst -> Subst.
 
-Axiom extendSubstWithVar : Subst -> CoreType.Var -> CoreType.Var -> Subst.
+Axiom extendSubstWithVar : Subst -> Var.Var -> Var.Var -> Subst.
 
-Axiom extendSubstList : Subst ->
-                        list (CoreType.Var * CoreSyn.CoreArg)%type -> Subst.
+Axiom extendSubstList : Subst -> list (Var.Var * CoreSyn.CoreArg)%type -> Subst.
 
-Axiom extendSubst : Subst -> CoreType.Var -> CoreSyn.CoreArg -> Subst.
+Axiom extendSubst : Subst -> Var.Var -> CoreSyn.CoreArg -> Subst.
 
-Axiom extendIdSubst : Subst -> CoreType.Id -> CoreSyn.CoreExpr -> Subst.
+Axiom extendIdSubst : Subst -> Var.Id -> CoreSyn.CoreExpr -> Subst.
 
 Axiom extendIdSubstList : Subst ->
-                          list (CoreType.Id * CoreSyn.CoreExpr)%type -> Subst.
+                          list (Var.Id * CoreSyn.CoreExpr)%type -> Subst.
 
-Axiom extendTvSubstList : Subst ->
-                          list (CoreType.TyVar * CoreType.Type_)%type -> Subst.
+Axiom extendTvSubstList : Subst -> list (Var.TyVar * unit)%type -> Subst.
 
-Axiom extendTvSubst : Subst -> CoreType.TyVar -> CoreType.Type_ -> Subst.
+Axiom extendTvSubst : Subst -> Var.TyVar -> unit -> Subst.
 
-Axiom extendCvSubst : Subst -> CoreType.CoVar -> CoreType.Coercion -> Subst.
+Axiom extendCvSubst : Subst -> Var.CoVar -> unit -> Subst.
 
 Axiom substRulesForImportedIds : Subst ->
                                  list CoreSyn.CoreRule -> list CoreSyn.CoreRule.
 
 Axiom cloneRecIdBndrs : Subst ->
-                        UniqSupply.UniqSupply -> list CoreType.Id -> (Subst * list CoreType.Id)%type.
+                        UniqSupply.UniqSupply -> list Var.Id -> (Subst * list Var.Id)%type.
 
 Axiom cloneBndrs : Subst ->
-                   UniqSupply.UniqSupply -> list CoreType.Var -> (Subst * list CoreType.Var)%type.
+                   UniqSupply.UniqSupply -> list Var.Var -> (Subst * list Var.Var)%type.
 
-Axiom cloneBndr : Subst ->
-                  Unique.Unique -> CoreType.Var -> (Subst * CoreType.Var)%type.
+Axiom cloneBndr : Subst -> Unique.Unique -> Var.Var -> (Subst * Var.Var)%type.
 
 Axiom cloneIdBndrs : Subst ->
-                     UniqSupply.UniqSupply -> list CoreType.Id -> (Subst * list CoreType.Id)%type.
+                     UniqSupply.UniqSupply -> list Var.Id -> (Subst * list Var.Id)%type.
 
 Axiom cloneIdBndr : Subst ->
-                    UniqSupply.UniqSupply -> CoreType.Id -> (Subst * CoreType.Id)%type.
+                    UniqSupply.UniqSupply -> Var.Id -> (Subst * Var.Id)%type.
 
 Axiom clone_id : Subst ->
-                 Subst -> (CoreType.Id * Unique.Unique)%type -> (Subst * CoreType.Id)%type.
+                 Subst -> (Var.Id * Unique.Unique)%type -> (Subst * Var.Id)%type.
 
-Axiom substRecBndrs : Subst ->
-                      list CoreType.Id -> (Subst * list CoreType.Id)%type.
+Axiom substRecBndrs : Subst -> list Var.Id -> (Subst * list Var.Id)%type.
 
 Axiom substRule : Subst ->
                   (Name.Name -> Name.Name) -> CoreSyn.CoreRule -> CoreSyn.CoreRule.
 
-Axiom substSpec : Subst -> CoreType.Id -> IdInfo.RuleInfo -> IdInfo.RuleInfo.
+Axiom substSpec : Subst -> Var.Id -> IdInfo.RuleInfo -> IdInfo.RuleInfo.
 
-Axiom substBndrs : Subst ->
-                   list CoreType.Var -> (Subst * list CoreType.Var)%type.
+Axiom substBndrs : Subst -> list Var.Var -> (Subst * list Var.Var)%type.
 
 Axiom substExpr : unit -> Subst -> CoreSyn.CoreExpr -> CoreSyn.CoreExpr.
 
 Axiom substUnfolding : Subst -> CoreSyn.Unfolding -> CoreSyn.Unfolding.
 
-Axiom substIdInfo : Subst ->
-                    CoreType.Id -> IdInfo.IdInfo -> option IdInfo.IdInfo.
+Axiom substIdInfo : Subst -> Var.Id -> IdInfo.IdInfo -> option IdInfo.IdInfo.
 
-Axiom substIdBndr : unit ->
-                    Subst -> Subst -> CoreType.Id -> (Subst * CoreType.Id)%type.
+Axiom substIdBndr : unit -> Subst -> Subst -> Var.Id -> (Subst * Var.Id)%type.
 
-Axiom substBndr : Subst -> CoreType.Var -> (Subst * CoreType.Var)%type.
+Axiom substBndr : Subst -> Var.Var -> (Subst * Var.Var)%type.
 
 Axiom substBind : Subst -> CoreSyn.CoreBind -> (Subst * CoreSyn.CoreBind)%type.
 
 Axiom subst_expr : unit -> Subst -> CoreSyn.CoreExpr -> CoreSyn.CoreExpr.
 
-Axiom substTickish : Subst ->
-                     CoreSyn.Tickish CoreType.Id -> CoreSyn.Tickish CoreType.Id.
+Axiom substTickish : Subst -> CoreSyn.Tickish Var.Id -> CoreSyn.Tickish Var.Id.
 
-Axiom substDVarSet : Subst -> CoreType.DVarSet -> CoreType.DVarSet.
+Axiom substDVarSet : Subst -> VarSet.DVarSet -> VarSet.DVarSet.
 
-Axiom substIdOcc : Subst -> CoreType.Id -> CoreType.Id.
+Axiom substIdOcc : Subst -> Var.Id -> Var.Id.
 
-Axiom lookupIdSubst : unit -> Subst -> CoreType.Id -> CoreSyn.CoreExpr.
+Axiom lookupIdSubst : unit -> Subst -> Var.Id -> CoreSyn.CoreExpr.
 
-Axiom lookupTCvSubst : Subst -> CoreType.TyVar -> CoreType.Type_.
+Axiom lookupTCvSubst : Subst -> Var.TyVar -> unit.
 
-Axiom delBndr : Subst -> CoreType.Var -> Subst.
+Axiom delBndr : Subst -> Var.Var -> Subst.
 
-Axiom delBndrs : Subst -> list CoreType.Var -> Subst.
+Axiom delBndrs : Subst -> list Var.Var -> Subst.
 
-Axiom mkOpenSubst : CoreType.InScopeSet ->
-                    list (CoreType.Var * CoreSyn.CoreArg)%type -> Subst.
+Axiom mkOpenSubst : VarEnv.InScopeSet ->
+                    list (Var.Var * CoreSyn.CoreArg)%type -> Subst.
 
-Axiom isInScope : CoreType.Var -> Subst -> bool.
+Axiom isInScope : Var.Var -> Subst -> bool.
 
-Axiom addInScopeSet : Subst -> CoreType.VarSet -> Subst.
+Axiom addInScopeSet : Subst -> VarSet.VarSet -> Subst.
 
-Axiom extendInScope : Subst -> CoreType.Var -> Subst.
+Axiom extendInScope : Subst -> Var.Var -> Subst.
 
-Axiom extendInScopeList : Subst -> list CoreType.Var -> Subst.
+Axiom extendInScopeList : Subst -> list Var.Var -> Subst.
 
-Axiom extendInScopeIds : Subst -> list CoreType.Id -> Subst.
+Axiom extendInScopeIds : Subst -> list Var.Id -> Subst.
 
-Axiom setInScope : Subst -> CoreType.InScopeSet -> Subst.
+Axiom setInScope : Subst -> VarEnv.InScopeSet -> Subst.
 
-Axiom substTyVarBndr : Subst -> CoreType.TyVar -> (Subst * CoreType.TyVar)%type.
+Axiom substTyVarBndr : Subst -> Var.TyVar -> (Subst * Var.TyVar)%type.
 
 Axiom cloneTyVarBndr : Subst ->
-                       CoreType.TyVar -> Unique.Unique -> (Subst * CoreType.TyVar)%type.
+                       Var.TyVar -> Unique.Unique -> (Subst * Var.TyVar)%type.
 
-Axiom substCoVarBndr : Subst -> CoreType.TyVar -> (Subst * CoreType.TyVar)%type.
+Axiom substCoVarBndr : Subst -> Var.TyVar -> (Subst * Var.TyVar)%type.
 
-Axiom substIdType : Subst -> CoreType.Id -> CoreType.Id.
+Axiom substIdType : Subst -> Var.Id -> Var.Id.
 
-Axiom substTy : Subst -> CoreType.Type_ -> CoreType.Type_.
+Axiom substTy : Subst -> unit -> unit.
 
-Axiom substCo : Subst -> CoreType.Coercion -> CoreType.Coercion.
+Axiom substCo : Subst -> unit -> unit.
 
-Axiom getTCvSubst : Subst -> CoreType.TCvSubst.
+Axiom getTCvSubst : Subst -> TyCoRep.TCvSubst.
 
 (* External variables:
      bool list op_zt__ option unit CoreSyn.CoreArg CoreSyn.CoreBind CoreSyn.CoreExpr
      CoreSyn.CoreProgram CoreSyn.CoreRule CoreSyn.Tickish CoreSyn.Unfolding
-     CoreType.CoVar CoreType.Coercion CoreType.CvSubstEnv CoreType.DVarSet
-     CoreType.Id CoreType.IdEnv CoreType.InScopeSet CoreType.TCvSubst
-     CoreType.TvSubstEnv CoreType.TyVar CoreType.Type_ CoreType.Var CoreType.VarSet
-     IdInfo.IdInfo IdInfo.RuleInfo Name.Name UniqSupply.UniqSupply Unique.Unique
+     IdInfo.IdInfo IdInfo.RuleInfo Name.Name TyCoRep.CvSubstEnv TyCoRep.TCvSubst
+     TyCoRep.TvSubstEnv UniqSupply.UniqSupply Unique.Unique Var.CoVar Var.Id
+     Var.TyVar Var.Var VarEnv.IdEnv VarEnv.InScopeSet VarSet.DVarSet VarSet.VarSet
 *)
