examples/ghc/lib/FV.v
@@ -12,6 +12,8 @@ Require Coq.Program.Wf.
 
 (* Preamble *)
 
+
+
 (* Converted imports: *)
 
 Require Data.Tuple.
