examples/ghc/lib/Id.v
@@ -18,24 +18,22 @@ Require Panic.
 
 Require BasicTypes.
 Require CoreSyn.
-Require CoreType.
 Require DataCon.
 Require Demand.
 Require FastString.
 Require GHC.Base.
 Require GHC.Num.
 Require IdInfo.
-Require IdInfo2.
 Require Maybes.
 Require Module.
 Require Name.
 Require OccName.
 Require Panic.
-Require RepType.
 Require SrcLoc.
 Require UniqSupply.
 Require Unique.
 Require Util.
+Require Var.
 Import GHC.Base.Notations.
 Import GHC.Num.Notations.
 
@@ -45,7 +43,6 @@ Import GHC.Num.Notations.
 (* Record selectors *)
 Import IdInfo.
 Import IdInfo2.
-Import Core.
 
 Parameter hasNoBinding : Var.Id -> bool.
 
@@ -105,95 +102,95 @@ Axiom asJoinId : forall {A : Type}, A.
 (* Translating `asJoinId' failed: using a record pattern for the unknown
    constructor `JoinId' unsupported *)
 
-Definition idArity : CoreType.Id -> BasicTypes.Arity :=
-  fun id => IdInfo.arityInfo (CoreType.idInfo id).
+Definition idArity : Var.Id -> BasicTypes.Arity :=
+  fun id => IdInfo.arityInfo (Var.idInfo id).
 
-Definition idCafInfo : CoreType.Id -> IdInfo.CafInfo :=
-  fun id => IdInfo.cafInfo (CoreType.idInfo id).
+Definition idCafInfo : Var.Id -> IdInfo.CafInfo :=
+  fun id => IdInfo.cafInfo (Var.idInfo id).
 
-Definition idCallArity : CoreType.Id -> BasicTypes.Arity :=
-  fun id => IdInfo.callArityInfo (CoreType.idInfo id).
+Definition idCallArity : Var.Id -> BasicTypes.Arity :=
+  fun id => IdInfo.callArityInfo (Var.idInfo id).
 
-Definition idDataCon : CoreType.Id -> DataCon.DataCon :=
+Definition idDataCon : Var.Id -> DataCon.DataCon :=
   fun id =>
     Maybes.orElse (isDataConId_maybe id) (Panic.panicStr (GHC.Base.hs_string__
                                                           "idDataCon") (Panic.noString id)).
 
-Definition idDemandInfo : CoreType.Id -> Demand.Demand :=
-  fun id => IdInfo2.demandInfo (CoreType.idInfo id).
+Definition idDemandInfo : Var.Id -> Demand.Demand :=
+  fun id => IdInfo.demandInfo (Var.idInfo id).
 
-Definition idInlinePragma : CoreType.Id -> BasicTypes.InlinePragma :=
-  fun id => IdInfo.inlinePragInfo (CoreType.idInfo id).
+Definition idInlinePragma : Var.Id -> BasicTypes.InlinePragma :=
+  fun id => IdInfo.inlinePragInfo (Var.idInfo id).
 
-Definition idRuleMatchInfo : CoreType.Id -> BasicTypes.RuleMatchInfo :=
+Definition idRuleMatchInfo : Var.Id -> BasicTypes.RuleMatchInfo :=
   fun id => BasicTypes.inlinePragmaRuleMatchInfo (idInlinePragma id).
 
-Definition isConLikeId : CoreType.Id -> bool :=
+Definition isConLikeId : Var.Id -> bool :=
   fun id => orb (isDataConWorkId id) (BasicTypes.isConLike (idRuleMatchInfo id)).
 
-Definition idInlineActivation : CoreType.Id -> BasicTypes.Activation :=
+Definition idInlineActivation : Var.Id -> BasicTypes.Activation :=
   fun id => BasicTypes.inlinePragmaActivation (idInlinePragma id).
 
-Definition idName : CoreType.Id -> Name.Name :=
-  CoreType.varName.
+Definition idName : Var.Id -> Name.Name :=
+  Var.varName.
 
-Definition idIsFrom : Module.Module -> CoreType.Id -> bool :=
+Definition idIsFrom : Module.Module -> Var.Id -> bool :=
   fun mod_ id => Name.nameIsLocalOrFrom mod_ (idName id).
 
-Definition idOccInfo : CoreType.Id -> BasicTypes.OccInfo :=
-  fun id => IdInfo.occInfo (CoreType.idInfo id).
+Definition idOccInfo : Var.Id -> BasicTypes.OccInfo :=
+  fun id => IdInfo.occInfo (Var.idInfo id).
 
-Definition isDeadBinder : CoreType.Id -> bool :=
+Definition isDeadBinder : Var.Id -> bool :=
   fun bndr =>
-    if CoreType.isId bndr : bool then BasicTypes.isDeadOcc (idOccInfo bndr) else
+    if Var.isId bndr : bool then BasicTypes.isDeadOcc (idOccInfo bndr) else
     false.
 
-Definition idOneShotInfo : CoreType.Id -> BasicTypes.OneShotInfo :=
-  fun id => IdInfo.oneShotInfo (CoreType.idInfo id).
+Definition idOneShotInfo : Var.Id -> BasicTypes.OneShotInfo :=
+  fun id => IdInfo.oneShotInfo (Var.idInfo id).
 
-Definition idSpecialisation : CoreType.Id -> IdInfo.RuleInfo :=
-  fun id => IdInfo.ruleInfo (CoreType.idInfo id).
+Definition idSpecialisation : Var.Id -> IdInfo.RuleInfo :=
+  fun id => IdInfo.ruleInfo (Var.idInfo id).
 
-Definition idHasRules : CoreType.Id -> bool :=
+Definition idHasRules : Var.Id -> bool :=
   fun id => negb (IdInfo.isEmptyRuleInfo (idSpecialisation id)).
 
-Definition idCoreRules : CoreType.Id -> list CoreSyn.CoreRule :=
-  fun id => IdInfo2.ruleInfoRules (idSpecialisation id).
+Definition idCoreRules : Var.Id -> list CoreSyn.CoreRule :=
+  fun id => IdInfo.ruleInfoRules (idSpecialisation id).
 
-Definition idStrictness : CoreType.Id -> Demand.StrictSig :=
-  fun id => IdInfo2.strictnessInfo (CoreType.idInfo id).
+Definition idStrictness : Var.Id -> Demand.StrictSig :=
+  fun id => IdInfo.strictnessInfo (Var.idInfo id).
 
-Definition isBottomingId : CoreType.Var -> bool :=
+Definition isBottomingId : Var.Var -> bool :=
   fun v =>
-    if CoreType.isId v : bool then Demand.isBottomingSig (idStrictness v) else
+    if Var.isId v : bool then Demand.isBottomingSig (idStrictness v) else
     false.
 
-Definition idType : CoreType.Id -> CoreType.Kind :=
-  CoreType.varType.
+Definition idType : Var.Id -> unit :=
+  Var.varType.
 
-Definition localiseId : CoreType.Id -> CoreType.Id :=
+Definition localiseId : Var.Id -> Var.Id :=
   fun id =>
     let name := idName id in
-    if (if andb Util.debugIsOn (negb (CoreType.isId id)) : bool
+    if (if andb Util.debugIsOn (negb (Var.isId id)) : bool
         then (Panic.assertPanic (GHC.Base.hs_string__ "ghc/compiler/basicTypes/Id.hs")
               #209)
-        else andb (CoreType.isLocalId id) (Name.isInternalName name)) : bool
+        else andb (Var.isLocalId id) (Name.isInternalName name)) : bool
     then id else
-    CoreType.mkLocalVar (CoreType.idDetails id) (Name.localiseName name) (idType id)
-    (CoreType.idInfo id).
+    Var.mkLocalVar (Var.idDetails id) (Name.localiseName name) (idType id)
+    (Var.idInfo id).
 
-Definition idFunRepArity : CoreType.Id -> BasicTypes.RepArity :=
+Definition idFunRepArity : Var.Id -> BasicTypes.RepArity :=
   fun x => RepType.countFunRepArgs (idArity x) (idType x).
 
-Definition idUnfolding : CoreType.Id -> CoreSyn.Unfolding :=
+Definition idUnfolding : Var.Id -> CoreSyn.Unfolding :=
   fun id =>
-    let info := CoreType.idInfo id in
+    let info := Var.idInfo id in
     if BasicTypes.isStrongLoopBreaker (IdInfo.occInfo info) : bool
     then CoreSyn.NoUnfolding else
-    IdInfo2.unfoldingInfo info.
+    IdInfo.unfoldingInfo info.
 
-Definition idUnique : CoreType.Id -> Unique.Unique :=
-  CoreType.varUnique.
+Definition idUnique : Var.Id -> Unique.Unique :=
+  Var.varUnique.
 
 Axiom isDFunId : forall {A : Type}, A.
 
@@ -212,7 +209,7 @@ Axiom isImplicitId : forall {A : Type}, A.
 
 Axiom isJoinId : forall {A : Type}, A.
 
-Definition isExitJoinId : CoreType.Var -> bool :=
+Definition isExitJoinId : Var.Var -> bool :=
   fun id =>
     andb (isJoinId id) (andb (BasicTypes.isOneOcc (idOccInfo id))
                              (BasicTypes.occ_in_lam (idOccInfo id))).
@@ -220,19 +217,19 @@ Definition isExitJoinId : CoreType.Var -> bool :=
 (* Translating `isJoinId' failed: using a record pattern for the unknown
    constructor `JoinId' unsupported *)
 
-Definition isJoinId_maybe : CoreType.Var -> option BasicTypes.JoinArity :=
+Definition isJoinId_maybe : Var.Var -> option BasicTypes.JoinArity :=
   fun id =>
-    if CoreType.isId id : bool
-    then if andb Util.debugIsOn (negb (CoreType.isId id)) : bool
+    if Var.isId id : bool
+    then if andb Util.debugIsOn (negb (Var.isId id)) : bool
          then (Outputable.assertPprPanic (GHC.Base.hs_string__
                                           "ghc/compiler/basicTypes/Id.hs") #494 (Panic.noString id))
-         else match CoreType.idDetails id with
+         else match Var.idDetails id with
               | IdInfo.JoinId arity => Some arity
               | _ => None
               end else
     None.
 
-Definition idJoinArity : CoreType.JoinId -> BasicTypes.JoinArity :=
+Definition idJoinArity : Var.JoinId -> BasicTypes.JoinArity :=
   fun id =>
     Maybes.orElse (isJoinId_maybe id) (Panic.panicStr (GHC.Base.hs_string__
                                                        "idJoinArity") (Panic.noString id)).
@@ -242,8 +239,8 @@ Axiom isNaughtyRecordSelector : forall {A : Type}, A.
 (* Translating `isNaughtyRecordSelector' failed: using a record pattern for the
    unknown constructor `RecSelId' unsupported *)
 
-Definition isNeverLevPolyId : CoreType.Id -> bool :=
-  IdInfo.isNeverLevPolyIdInfo GHC.Base.∘ CoreType.idInfo.
+Definition isNeverLevPolyId : Var.Id -> bool :=
+  IdInfo.isNeverLevPolyIdInfo GHC.Base.∘ Var.idInfo.
 
 Axiom isPatSynRecordSelector : forall {A : Type}, A.
 
@@ -255,11 +252,10 @@ Axiom isRecordSelector : forall {A : Type}, A.
 (* Translating `isRecordSelector' failed: using a record pattern for the unknown
    constructor `RecSelId' unsupported *)
 
-Definition lazySetIdInfo : CoreType.Id -> IdInfo.IdInfo -> CoreType.Id :=
-  CoreType.lazySetIdInfo.
+Definition lazySetIdInfo : Var.Id -> IdInfo.IdInfo -> Var.Id :=
+  Var.lazySetIdInfo.
 
-Definition maybeModifyIdInfo
-   : option IdInfo.IdInfo -> CoreType.Id -> CoreType.Id :=
+Definition maybeModifyIdInfo : option IdInfo.IdInfo -> Var.Id -> Var.Id :=
   fun arg_0__ arg_1__ =>
     match arg_0__, arg_1__ with
     | Some new_info, id => lazySetIdInfo id new_info
@@ -267,94 +263,88 @@ Definition maybeModifyIdInfo
     end.
 
 Definition zapInfo
-   : (IdInfo.IdInfo -> option IdInfo.IdInfo) -> CoreType.Id -> CoreType.Id :=
-  fun zapper id => maybeModifyIdInfo (zapper (CoreType.idInfo id)) id.
+   : (IdInfo.IdInfo -> option IdInfo.IdInfo) -> Var.Id -> Var.Id :=
+  fun zapper id => maybeModifyIdInfo (zapper (Var.idInfo id)) id.
 
-Definition zapFragileIdInfo : CoreType.Id -> CoreType.Id :=
+Definition zapFragileIdInfo : Var.Id -> Var.Id :=
   zapInfo IdInfo.zapFragileInfo.
 
-Definition zapIdDemandInfo : CoreType.Id -> CoreType.Id :=
+Definition zapIdDemandInfo : Var.Id -> Var.Id :=
   zapInfo IdInfo.zapDemandInfo.
 
-Definition zapIdTailCallInfo : CoreType.Id -> CoreType.Id :=
+Definition zapIdTailCallInfo : Var.Id -> Var.Id :=
   zapInfo IdInfo.zapTailCallInfo.
 
-Definition zapJoinId : CoreType.Id -> CoreType.Id :=
+Definition zapJoinId : Var.Id -> Var.Id :=
   fun jid =>
     if isJoinId jid : bool
-    then zapIdTailCallInfo (CoreType.setIdDetails jid IdInfo.VanillaId) else
+    then zapIdTailCallInfo (Var.setIdDetails jid IdInfo.VanillaId) else
     jid.
 
-Definition asJoinId_maybe
-   : CoreType.Id -> option BasicTypes.JoinArity -> CoreType.Id :=
+Definition asJoinId_maybe : Var.Id -> option BasicTypes.JoinArity -> Var.Id :=
   fun arg_0__ arg_1__ =>
     match arg_0__, arg_1__ with
     | id, Some arity => asJoinId id arity
     | id, None => zapJoinId id
     end.
 
-Definition zapIdUsageEnvInfo : CoreType.Id -> CoreType.Id :=
+Definition zapIdUsageEnvInfo : Var.Id -> Var.Id :=
   zapInfo IdInfo.zapUsageEnvInfo.
 
-Definition zapIdUsageInfo : CoreType.Id -> CoreType.Id :=
+Definition zapIdUsageInfo : Var.Id -> Var.Id :=
   zapInfo IdInfo.zapUsageInfo.
 
-Definition zapIdUsedOnceInfo : CoreType.Id -> CoreType.Id :=
+Definition zapIdUsedOnceInfo : Var.Id -> Var.Id :=
   zapInfo IdInfo.zapUsedOnceInfo.
 
-Definition zapLamIdInfo : CoreType.Id -> CoreType.Id :=
+Definition zapLamIdInfo : Var.Id -> Var.Id :=
   zapInfo IdInfo.zapLamInfo.
 
-Definition setIdInfo : CoreType.Id -> IdInfo.IdInfo -> CoreType.Id :=
+Definition setIdInfo : Var.Id -> IdInfo.IdInfo -> Var.Id :=
   fun id info => lazySetIdInfo id info.
 
 Definition modifyIdInfo
-   : (IdInfo.IdInfo -> IdInfo.IdInfo) -> CoreType.Id -> CoreType.Id :=
-  fun fn id => setIdInfo id (fn (CoreType.idInfo id)).
+   : (IdInfo.IdInfo -> IdInfo.IdInfo) -> Var.Id -> Var.Id :=
+  fun fn id => setIdInfo id (fn (Var.idInfo id)).
 
 Definition modifyInlinePragma
-   : CoreType.Id ->
-     (BasicTypes.InlinePragma -> BasicTypes.InlinePragma) -> CoreType.Id :=
+   : Var.Id -> (BasicTypes.InlinePragma -> BasicTypes.InlinePragma) -> Var.Id :=
   fun id fn =>
     modifyIdInfo (fun info =>
                     IdInfo.setInlinePragInfo info (fn (IdInfo.inlinePragInfo info))) id.
 
-Definition setInlineActivation
-   : CoreType.Id -> BasicTypes.Activation -> CoreType.Id :=
+Definition setInlineActivation : Var.Id -> BasicTypes.Activation -> Var.Id :=
   fun id act =>
     modifyInlinePragma id (fun prag =>
                              BasicTypes.setInlinePragmaActivation prag act).
 
-Definition setIdArity : CoreType.Id -> BasicTypes.Arity -> CoreType.Id :=
+Definition setIdArity : Var.Id -> BasicTypes.Arity -> Var.Id :=
   fun id arity =>
     modifyIdInfo (fun arg_0__ => IdInfo.setArityInfo arg_0__ arity) id.
 
-Definition setIdCafInfo : CoreType.Id -> IdInfo.CafInfo -> CoreType.Id :=
+Definition setIdCafInfo : Var.Id -> IdInfo.CafInfo -> Var.Id :=
   fun id caf_info =>
     modifyIdInfo (fun arg_0__ => IdInfo.setCafInfo arg_0__ caf_info) id.
 
-Definition setIdCallArity : CoreType.Id -> BasicTypes.Arity -> CoreType.Id :=
+Definition setIdCallArity : Var.Id -> BasicTypes.Arity -> Var.Id :=
   fun id arity =>
     modifyIdInfo (fun arg_0__ => IdInfo.setCallArityInfo arg_0__ arity) id.
 
-Definition setIdDemandInfo : CoreType.Id -> Demand.Demand -> CoreType.Id :=
-  fun id dmd =>
-    modifyIdInfo (fun arg_0__ => IdInfo2.setDemandInfo arg_0__ dmd) id.
+Definition setIdDemandInfo : Var.Id -> Demand.Demand -> Var.Id :=
+  fun id dmd => modifyIdInfo (fun arg_0__ => IdInfo.setDemandInfo arg_0__ dmd) id.
 
-Definition setIdOccInfo : CoreType.Id -> BasicTypes.OccInfo -> CoreType.Id :=
+Definition setIdOccInfo : Var.Id -> BasicTypes.OccInfo -> Var.Id :=
   fun id occ_info =>
     modifyIdInfo (fun arg_0__ => IdInfo.setOccInfo arg_0__ occ_info) id.
 
-Definition zapIdOccInfo : CoreType.Id -> CoreType.Id :=
+Definition zapIdOccInfo : Var.Id -> Var.Id :=
   fun b => setIdOccInfo b BasicTypes.noOccInfo.
 
-Definition setIdOneShotInfo
-   : CoreType.Id -> BasicTypes.OneShotInfo -> CoreType.Id :=
+Definition setIdOneShotInfo : Var.Id -> BasicTypes.OneShotInfo -> Var.Id :=
   fun id one_shot =>
     modifyIdInfo (fun arg_0__ => IdInfo.setOneShotInfo arg_0__ one_shot) id.
 
-Definition updOneShotInfo
-   : CoreType.Id -> BasicTypes.OneShotInfo -> CoreType.Id :=
+Definition updOneShotInfo : Var.Id -> BasicTypes.OneShotInfo -> Var.Id :=
   fun id one_shot =>
     let do_upd :=
       match pair (idOneShotInfo id) one_shot with
@@ -364,124 +354,115 @@ Definition updOneShotInfo
     if do_upd : bool then setIdOneShotInfo id one_shot else
     id.
 
-Definition setIdSpecialisation
-   : CoreType.Id -> IdInfo.RuleInfo -> CoreType.Id :=
+Definition setIdSpecialisation : Var.Id -> IdInfo.RuleInfo -> Var.Id :=
   fun id spec_info =>
     modifyIdInfo (fun arg_0__ => IdInfo.setRuleInfo arg_0__ spec_info) id.
 
-Definition setIdStrictness : CoreType.Id -> Demand.StrictSig -> CoreType.Id :=
+Definition setIdStrictness : Var.Id -> Demand.StrictSig -> Var.Id :=
   fun id sig =>
-    modifyIdInfo (fun arg_0__ => IdInfo2.setStrictnessInfo arg_0__ sig) id.
+    modifyIdInfo (fun arg_0__ => IdInfo.setStrictnessInfo arg_0__ sig) id.
 
-Definition setIdUnfolding : CoreType.Id -> CoreSyn.Unfolding -> CoreType.Id :=
+Definition setIdUnfolding : Var.Id -> CoreSyn.Unfolding -> Var.Id :=
   fun id unfolding =>
-    modifyIdInfo (fun arg_0__ => IdInfo2.setUnfoldingInfo arg_0__ unfolding) id.
+    modifyIdInfo (fun arg_0__ => IdInfo.setUnfoldingInfo arg_0__ unfolding) id.
 
-Definition setCaseBndrEvald
-   : DataCon.StrictnessMark -> CoreType.Id -> CoreType.Id :=
+Definition setCaseBndrEvald : DataCon.StrictnessMark -> Var.Id -> Var.Id :=
   fun str id =>
     if DataCon.isMarkedStrict str : bool
     then setIdUnfolding id CoreSyn.evaldUnfolding else
     id.
 
-Definition setInlinePragma
-   : CoreType.Id -> BasicTypes.InlinePragma -> CoreType.Id :=
+Definition setInlinePragma : Var.Id -> BasicTypes.InlinePragma -> Var.Id :=
   fun id prag =>
     modifyIdInfo (fun arg_0__ => IdInfo.setInlinePragInfo arg_0__ prag) id.
 
-Definition setOneShotLambda : CoreType.Id -> CoreType.Id :=
+Definition setOneShotLambda : Var.Id -> Var.Id :=
   fun id =>
     modifyIdInfo (fun arg_0__ =>
                     IdInfo.setOneShotInfo arg_0__ BasicTypes.OneShotLam) id.
 
-Definition transferPolyIdInfo
-   : CoreType.Id -> list CoreType.Var -> CoreType.Id -> CoreType.Id :=
+Definition transferPolyIdInfo : Var.Id -> list Var.Var -> Var.Id -> Var.Id :=
   fun old_id abstract_wrt new_id =>
-    let old_info := CoreType.idInfo old_id in
+    let old_info := Var.idInfo old_id in
     let old_arity := IdInfo.arityInfo old_info in
     let old_inline_prag := IdInfo.inlinePragInfo old_info in
     let old_occ_info := IdInfo.occInfo old_info in
     let new_occ_info := BasicTypes.zapOccTailCallInfo old_occ_info in
-    let old_strictness := IdInfo2.strictnessInfo old_info in
-    let arity_increase := Util.count CoreType.isId abstract_wrt in
+    let old_strictness := IdInfo.strictnessInfo old_info in
+    let arity_increase := Util.count Var.isId abstract_wrt in
     let new_arity := old_arity GHC.Num.+ arity_increase in
     let new_strictness :=
       Demand.increaseStrictSigArity arity_increase old_strictness in
     let transfer :=
       fun new_info =>
-        IdInfo2.setStrictnessInfo (IdInfo.setOccInfo (IdInfo.setInlinePragInfo
-                                                      (IdInfo.setArityInfo new_info new_arity) old_inline_prag)
-                                                     new_occ_info) new_strictness in
+        IdInfo.setStrictnessInfo (IdInfo.setOccInfo (IdInfo.setInlinePragInfo
+                                                     (IdInfo.setArityInfo new_info new_arity) old_inline_prag)
+                                                    new_occ_info) new_strictness in
     modifyIdInfo transfer new_id.
 
-Definition zapIdStrictness : CoreType.Id -> CoreType.Id :=
+Definition zapIdStrictness : Var.Id -> Var.Id :=
   fun id =>
-    modifyIdInfo (fun arg_0__ => IdInfo2.setStrictnessInfo arg_0__ Demand.nopSig)
-    id.
+    modifyIdInfo (fun arg_0__ => IdInfo.setStrictnessInfo arg_0__ Demand.nopSig) id.
 
-Definition clearOneShotLambda : CoreType.Id -> CoreType.Id :=
+Definition clearOneShotLambda : Var.Id -> Var.Id :=
   fun id =>
     modifyIdInfo (fun arg_0__ =>
                     IdInfo.setOneShotInfo arg_0__ BasicTypes.NoOneShotInfo) id.
 
 Definition mkExportedLocalId
-   : IdInfo.IdDetails -> Name.Name -> CoreType.Type_ -> CoreType.Id :=
+   : IdInfo.IdDetails -> Name.Name -> unit -> Var.Id :=
   fun details name ty =>
-    CoreType.mkExportedLocalVar details name ty IdInfo.vanillaIdInfo.
+    Var.mkExportedLocalVar details name ty IdInfo.vanillaIdInfo.
 
 Definition mkGlobalId
-   : IdInfo.IdDetails ->
-     Name.Name -> CoreType.Type_ -> IdInfo.IdInfo -> CoreType.Id :=
-  CoreType.mkGlobalVar.
+   : IdInfo.IdDetails -> Name.Name -> unit -> IdInfo.IdInfo -> Var.Id :=
+  Var.mkGlobalVar.
 
 Definition mkSysLocalM {m} `{UniqSupply.MonadUnique m}
-   : FastString.FastString -> CoreType.Type_ -> m CoreType.Id :=
+   : FastString.FastString -> unit -> m Var.Id :=
   fun fs ty =>
     UniqSupply.getUniqueM GHC.Base.>>=
     (fun uniq => GHC.Base.return_ (mkSysLocal fs uniq ty)).
 
 Definition mkSysLocalOrCoVar
-   : FastString.FastString -> Unique.Unique -> CoreType.Type_ -> CoreType.Id :=
+   : FastString.FastString -> Unique.Unique -> unit -> Var.Id :=
   fun fs uniq ty => mkLocalIdOrCoVar (Name.mkSystemVarName uniq fs) ty.
 
 Definition mkSysLocalOrCoVarM {m} `{UniqSupply.MonadUnique m}
-   : FastString.FastString -> CoreType.Type_ -> m CoreType.Id :=
+   : FastString.FastString -> unit -> m Var.Id :=
   fun fs ty =>
     UniqSupply.getUniqueM GHC.Base.>>=
     (fun uniq => GHC.Base.return_ (mkSysLocalOrCoVar fs uniq ty)).
 
-Definition mkTemplateLocal : GHC.Num.Int -> CoreType.Type_ -> CoreType.Id :=
+Definition mkTemplateLocal : GHC.Num.Int -> unit -> Var.Id :=
   fun i ty =>
     mkSysLocalOrCoVar (FastString.fsLit (GHC.Base.hs_string__ "v"))
     (Unique.mkBuiltinUnique i) ty.
 
-Definition mkTemplateLocals : list CoreType.Type_ -> list CoreType.Id :=
+Definition mkTemplateLocals : list unit -> list Var.Id :=
   mkTemplateLocalsNum #1.
 
 Definition mkUserLocal
-   : OccName.OccName ->
-     Unique.Unique -> CoreType.Type_ -> SrcLoc.SrcSpan -> CoreType.Id :=
+   : OccName.OccName -> Unique.Unique -> unit -> SrcLoc.SrcSpan -> Var.Id :=
   fun occ uniq ty loc =>
-    if andb Util.debugIsOn (negb (negb (CoreType.isCoercionType ty))) : bool
+    if andb Util.debugIsOn (negb (negb (TyCoRep.isCoercionType ty))) : bool
     then (Panic.assertPanic (GHC.Base.hs_string__ "ghc/compiler/basicTypes/Id.hs")
           #330)
     else mkLocalId (Name.mkInternalName uniq occ loc) ty.
 
 Definition mkUserLocalOrCoVar
-   : OccName.OccName ->
-     Unique.Unique -> CoreType.Type_ -> SrcLoc.SrcSpan -> CoreType.Id :=
+   : OccName.OccName -> Unique.Unique -> unit -> SrcLoc.SrcSpan -> Var.Id :=
   fun occ uniq ty loc => mkLocalIdOrCoVar (Name.mkInternalName uniq occ loc) ty.
 
-Definition mkWorkerId
-   : Unique.Unique -> CoreType.Id -> CoreType.Type_ -> CoreType.Id :=
+Definition mkWorkerId : Unique.Unique -> Var.Id -> unit -> Var.Id :=
   fun uniq unwrkr ty =>
     mkLocalIdOrCoVar (Name.mkDerivedInternalName OccName.mkWorkerOcc uniq
                       (Name.getName unwrkr)) ty.
 
-Definition realIdUnfolding : CoreType.Id -> CoreSyn.Unfolding :=
-  fun id => IdInfo2.unfoldingInfo (CoreType.idInfo id).
+Definition realIdUnfolding : Var.Id -> CoreSyn.Unfolding :=
+  fun id => IdInfo.unfoldingInfo (Var.idInfo id).
 
-Definition zapStableUnfolding : CoreType.Id -> CoreType.Id :=
+Definition zapStableUnfolding : Var.Id -> Var.Id :=
   fun id =>
     if CoreSyn.isStableUnfolding (realIdUnfolding id) : bool
     then setIdUnfolding id CoreSyn.NoUnfolding else
@@ -492,35 +473,35 @@ Axiom recordSelectorTyCon : forall {A : Type}, A.
 (* Translating `recordSelectorTyCon' failed: using a record pattern for the
    unknown constructor `RecSelId' unsupported *)
 
-Definition setIdExported : CoreType.Id -> CoreType.Id :=
-  CoreType.setIdExported.
+Definition setIdExported : Var.Id -> Var.Id :=
+  Var.setIdExported.
 
-Definition setIdName : CoreType.Id -> Name.Name -> CoreType.Id :=
-  CoreType.setVarName.
+Definition setIdName : Var.Id -> Name.Name -> Var.Id :=
+  Var.setVarName.
 
-Definition setIdNotExported : CoreType.Id -> CoreType.Id :=
-  CoreType.setIdNotExported.
+Definition setIdNotExported : Var.Id -> Var.Id :=
+  Var.setIdNotExported.
 
-Definition setIdUnique : CoreType.Id -> Unique.Unique -> CoreType.Id :=
-  CoreType.setVarUnique.
+Definition setIdUnique : Var.Id -> Unique.Unique -> Var.Id :=
+  Var.setVarUnique.
 
 Definition stateHackOneShot : BasicTypes.OneShotInfo :=
   BasicTypes.OneShotLam.
 
-Definition idStateHackOneShotInfo : CoreType.Id -> BasicTypes.OneShotInfo :=
+Definition idStateHackOneShotInfo : Var.Id -> BasicTypes.OneShotInfo :=
   fun id =>
     if isStateHackType (idType id) : bool then stateHackOneShot else
     idOneShotInfo id.
 
-Definition isOneShotBndr : CoreType.Var -> bool :=
+Definition isOneShotBndr : Var.Var -> bool :=
   fun var =>
-    if CoreType.isTyVar var : bool then true else
+    if Var.isTyVar var : bool then true else
     match idStateHackOneShotInfo var with
     | BasicTypes.OneShotLam => true
     | _ => false
     end.
 
-Definition isProbablyOneShotLambda : CoreType.Id -> bool :=
+Definition isProbablyOneShotLambda : Var.Id -> bool :=
   fun id =>
     match idStateHackOneShotInfo id with
     | BasicTypes.OneShotLam => true
@@ -530,7 +511,7 @@ Definition isProbablyOneShotLambda : CoreType.Id -> bool :=
 (* External variables:
      None Some andb bool false isDataConId_maybe isDataConWorkId isStateHackType list
      mkLocalId mkLocalIdOrCoVar mkSysLocal mkTemplateLocalsNum negb option orb pair
-     true BasicTypes.Activation BasicTypes.Arity BasicTypes.InlinePragma
+     true unit BasicTypes.Activation BasicTypes.Arity BasicTypes.InlinePragma
      BasicTypes.JoinArity BasicTypes.NoOneShotInfo BasicTypes.OccInfo
      BasicTypes.OneShotInfo BasicTypes.OneShotLam BasicTypes.RepArity
      BasicTypes.RuleMatchInfo BasicTypes.inlinePragmaActivation
@@ -538,33 +519,31 @@ Definition isProbablyOneShotLambda : CoreType.Id -> bool :=
      BasicTypes.isOneOcc BasicTypes.isStrongLoopBreaker BasicTypes.noOccInfo
      BasicTypes.occ_in_lam BasicTypes.setInlinePragmaActivation
      BasicTypes.zapOccTailCallInfo CoreSyn.CoreRule CoreSyn.NoUnfolding
-     CoreSyn.Unfolding CoreSyn.evaldUnfolding CoreSyn.isStableUnfolding CoreType.Id
-     CoreType.JoinId CoreType.Kind CoreType.Type_ CoreType.Var CoreType.idDetails
-     CoreType.idInfo CoreType.isCoercionType CoreType.isId CoreType.isLocalId
-     CoreType.isTyVar CoreType.lazySetIdInfo CoreType.mkExportedLocalVar
-     CoreType.mkGlobalVar CoreType.mkLocalVar CoreType.setIdDetails
-     CoreType.setIdExported CoreType.setIdNotExported CoreType.setVarName
-     CoreType.setVarUnique CoreType.varName CoreType.varType CoreType.varUnique
+     CoreSyn.Unfolding CoreSyn.evaldUnfolding CoreSyn.isStableUnfolding
      DataCon.DataCon DataCon.StrictnessMark DataCon.isMarkedStrict Demand.Demand
      Demand.StrictSig Demand.increaseStrictSigArity Demand.isBottomingSig
      Demand.nopSig FastString.FastString FastString.fsLit GHC.Base.op_z2218U__
      GHC.Base.op_zgzgze__ GHC.Base.return_ GHC.Num.Int GHC.Num.fromInteger
      GHC.Num.op_zp__ IdInfo.CafInfo IdInfo.IdDetails IdInfo.IdInfo IdInfo.JoinId
      IdInfo.RuleInfo IdInfo.VanillaId IdInfo.arityInfo IdInfo.cafInfo
-     IdInfo.callArityInfo IdInfo.inlinePragInfo IdInfo.isEmptyRuleInfo
-     IdInfo.isNeverLevPolyIdInfo IdInfo.occInfo IdInfo.oneShotInfo IdInfo.ruleInfo
-     IdInfo.setArityInfo IdInfo.setCafInfo IdInfo.setCallArityInfo
+     IdInfo.callArityInfo IdInfo.demandInfo IdInfo.inlinePragInfo
+     IdInfo.isEmptyRuleInfo IdInfo.isNeverLevPolyIdInfo IdInfo.occInfo
+     IdInfo.oneShotInfo IdInfo.ruleInfo IdInfo.ruleInfoRules IdInfo.setArityInfo
+     IdInfo.setCafInfo IdInfo.setCallArityInfo IdInfo.setDemandInfo
      IdInfo.setInlinePragInfo IdInfo.setOccInfo IdInfo.setOneShotInfo
-     IdInfo.setRuleInfo IdInfo.vanillaIdInfo IdInfo.zapDemandInfo
-     IdInfo.zapFragileInfo IdInfo.zapLamInfo IdInfo.zapTailCallInfo
-     IdInfo.zapUsageEnvInfo IdInfo.zapUsageInfo IdInfo.zapUsedOnceInfo
-     IdInfo2.demandInfo IdInfo2.ruleInfoRules IdInfo2.setDemandInfo
-     IdInfo2.setStrictnessInfo IdInfo2.setUnfoldingInfo IdInfo2.strictnessInfo
-     IdInfo2.unfoldingInfo Maybes.orElse Module.Module Name.Name Name.getName
+     IdInfo.setRuleInfo IdInfo.setStrictnessInfo IdInfo.setUnfoldingInfo
+     IdInfo.strictnessInfo IdInfo.unfoldingInfo IdInfo.vanillaIdInfo
+     IdInfo.zapDemandInfo IdInfo.zapFragileInfo IdInfo.zapLamInfo
+     IdInfo.zapTailCallInfo IdInfo.zapUsageEnvInfo IdInfo.zapUsageInfo
+     IdInfo.zapUsedOnceInfo Maybes.orElse Module.Module Name.Name Name.getName
      Name.isInternalName Name.localiseName Name.mkDerivedInternalName
      Name.mkInternalName Name.mkSystemVarName Name.nameIsLocalOrFrom OccName.OccName
      OccName.mkWorkerOcc Outputable.assertPprPanic Panic.assertPanic Panic.noString
-     Panic.panicStr RepType.countFunRepArgs SrcLoc.SrcSpan UniqSupply.MonadUnique
-     UniqSupply.getUniqueM Unique.Unique Unique.mkBuiltinUnique Util.count
-     Util.debugIsOn
+     Panic.panicStr RepType.countFunRepArgs SrcLoc.SrcSpan TyCoRep.isCoercionType
+     UniqSupply.MonadUnique UniqSupply.getUniqueM Unique.Unique
+     Unique.mkBuiltinUnique Util.count Util.debugIsOn Var.Id Var.JoinId Var.Var
+     Var.idDetails Var.idInfo Var.isId Var.isLocalId Var.isTyVar Var.lazySetIdInfo
+     Var.mkExportedLocalVar Var.mkGlobalVar Var.mkLocalVar Var.setIdDetails
+     Var.setIdExported Var.setIdNotExported Var.setVarName Var.setVarUnique
+     Var.varName Var.varType Var.varUnique
 *)
